@prefix owl: <http://www.w3.org/2002/07/owl#> .
@prefix rdf: <http://www.w3.org/1999/02/22-rdf-syntax-ns#> .
@prefix xsd: <http://www.w3.org/2001/XMLSchema#> .
@prefix airo: <https://w3id.org/airo#> .
@prefix rdfs: <http://www.w3.org/2000/01/rdf-schema#> .
@prefix terms: <http://purl.org/dc/terms/> .
@prefix earl: <http://www.w3.org/ns/earl#> .
@prefix dcat: <http://www.w3.org/ns/dcat#> .
@prefix dqv: <http://www.w3.org/ns/dqv#> .

@prefix : <https://example.org/ex#> .   # for new declarations

######################################
# Description of bias
######################################
:Bias rdf:type owl:Class ;
    terms:source "ISO/IEC 24027:2020, 3.3.2"@en ;
    rdfs:comment "systematic difference in treatment of certain objects, people, or groups in comparison to others."@en ;
    rdfs:label "bias"@en .

:CognitiveBias rdf:type owl:Class ;
    rdfs:subClassOf :Bias ;
    terms:source "ISO/IEC 24027:2020, 3.3.4"@en ;
    rdfs:comment "human bias that might impact the design and application of a system."@en ;
    rdfs:label "human cognitive bias"@en .

:AutomationBias rdf:type owl:Class ;
    rdfs:subClassOf :CognitiveBias ;
    terms:source "ISO/IEC 24027:2020, 3.3.1"@en ;
    rdfs:comment "type of human cognitive bias due to over-reliance on the recommendations of an AI system."@en ;
    rdfs:label "automation bias"@en .

:ConfirmationBias rdf:type owl:Class ;
    rdfs:subClassOf :CognitiveBias ;
    terms:source "ISO/IEC 24027:2020, 3.3.4"@en ;
    rdfs:comment "type of human cognitive bias that favours predictions of AI systems that confirm pre-existing beliefs or hypotheses."@en ;
    rdfs:label "confirmation bias"@en .

:DataBias rdf:type owl:Class ;
    terms:source "ISO/IEC 24027:2020, 3.3.7"@en ;
    rdfs:comment "data properties that if unaddressed lead to AI systems that perform better or worse for different groups."@en ;
    rdfs:label "data bias"@en .

:StatisticalBias rdf:type owl:Class ;
    terms:source "ISO 20501:2019, 3.3.9"@en ;
    rdfs:comment "type of consistent numerical offset in an estimate relative to the true underlying value, inherent to most estimates."@en ;
    rdfs:label "statistical bias"@en .

:Trustworthiness rdf:type airo:Entity ;
    terms:source "ISO 17068:2017, 3.18"@en ;
    rdfs:comment "quality of being dependable and reliable."@en ;
    rdfs:label "trustworthiness"@en .

:Group rdf:type owl:Class ;
    terms:source "ISO/IEC 24027:2020, 3.3.8"@en ;
    rdfs:comment "subset of objects in a domain that are linked because they have shared characteristics."@en ;
    rdfs:label "group"@en .


# The following are discussed in ISO/IEC 24027:2020 but not listed in the 'Terms' section of that document
:SocietalBias rdf:type owl:Class ;
    rdfs:subClassOf :CognitiveBias ;
    terms:source "ISO/IEC 24027:2020, 7.2.9"@en ;
    rdfs:comment "Societal bias occurs when one or more similar cognitive biases (conscious or unconscious) are being held by many individuals in society. This societal bias originates from society at large and could be closely related to other cognitive or statistical biases. It manifests as data available about society that reflects historical patterns. Societal bias can also be considered a type of data bias."@en ;
    rdfs:label "societal bias"@en .

:SelectionBias rdf:type owl:Class ;
    rdfs:subClassOf :DataBias ;
    terms:source "ISO/IEC 24027:2020, 7.3.2.1"@en ;
    rdfs:comment "Selection bias occurs when data is not collected randomly from the intended population."@en ;
    rdfs:label "selection bias"@en .

# Instance-level declarations of different types of societal bias.
:ReligionBias rdf:type :SocietalBias ;
    rdfs:comment "Bias related to a person's religion"@en ;
    rdfs:label "Religious bias"@en .

:RacialBias rdf:type :SocietalBias ;
    rdfs:comment "Bias related to the race of an individual"@en ;
    rdfs:label "Racial bias"@en .

:SexualOrientationBias rdf:type :SocietalBias ;
    rdfs:comment "Bias related to the sexual orientation of an individual"@en ;
    rdfs:label "Sexual orientation bias"@en .

:EthnicBias rdf:type :SocietalBias ;
    rdfs:comment "Bias related to the ethnicity of an individual"@en ;
    rdfs:label "Ethic bias"@en .

:PoliticalBias rdf:type :SocietalBias ;
    rdfs:comment "Bias related to political views"@en ;
    rdfs:label "Political bias"@en .

:PhilosophicalBeliefBias rdf:type :SocietalBias ;
    rdfs:comment "Bias related to philosophical beliefs"@en ;
    rdfs:label "Philophical belief bias"@en .

:TradeUnionMembershipBias rdf:type :SocietalBias ;
    rdfs:comment "Bias related to trade union membership"@en ;
    rdfs:label "Bias due to trade union membership"@en .

:GeneticDataBias rdf:type :SocietalBias ;
    rdfs:comment "Bias related to genetic data"@en ;
    rdfs:label "Genetic data bias"@en .

:BiometricDataUseBias rdf:type :SocietalBias ;
    rdfs:comment "Bias related to the use of biometric data"@en ;
    rdfs:label "Biometric data use bias"@en .

:HealthDataBias rdf:type :SocietalBias ;
    rdfs:comment "Bias related to health data"@en ;
    rdfs:label "Health data bias"@en .

# Added due to its importance; not listed in GDPR or ISO/IEC 24027:2020
:GenderBias rdf:type :SocietalBias ;
    rdfs:comment "Bias related to gender"@en ;
    rdfs:label "Gender bias"@en .

:SamplingBias rdf:type :SelectionBias ;
    terms:source "ISO/IEC 24027:2020, 7.3.2.2"@en ;
    rdfs:comment "Sampling bias occurs when data is not collected randomly from the intended population."@en ;
    rdfs:label "sampling bias"@en .

:CoverageBias rdf:type :SelectionBias ;
    terms:source "ISO/IEC 24027:2020, 7.3.2.3"@en ;
    rdfs:comment "Coverage bias occurs when a population represented in a dataset does not match the population that the ML model is making predictions about."@en ;
    rdfs:label "coverage bias"@en .

:NonResponseBias rdf:type :SelectionBias ;
    terms:source "ISO/IEC 24027:2020, 7.3.2.4"@en ;
    rdfs:comment "Non-response bias (also called participation bias) occurs when people from certain groups opt-out of surveys at different rates than users from other groups."@en ;
    rdfs:label "non-response bias"@en .

:DataLabelBias rdf:type :DataBias ;
    terms:source "ISO/IEC 24027:2020, 7.3.3"@en ;
    rdfs:comment "The labelling process itself potentially introduces the cognitive or societal biases described in subclause 7.2 to the data."@en ;
    rdfs:label "data labels and labelling process"@en .

:NonRepresentativeSampling rdf:type :DataBias ;
    terms:source "ISO/IEC 24027:2020, 7.3.4"@en ;
    rdfs:comment "If a dataset is not representative of the intended deployment environment, then the model has the potential to learn biases based on the ways in which the data is non-representative."@en ;
    rdfs:label "non-representative sampling"@en .

:MissingFeaturesLabels rdf:type :DataBias ;
    terms:source "ISO/IEC 24027:2020, 7.3.5"@en ;
    rdfs:comment "Features are often missing from individual training samples. If the frequency of missing features is higher for one group than another then this presents another vector for bias."@en ;
    rdfs:label "missing features and labels"@en .

:DataProcessing rdf:type :DataBias ;
    terms:source "ISO/IEC 24027:2020, 7.3.6"@en ;
    rdfs:comment "Bias might also creep in due to pre-processing (or post-processing) of data, even though the original data would not have led to any bias."@en ;
    rdfs:label "data processing bias"@en .

:SimpsonsParadox rdf:type :DataBias ;
    terms:source "ISO/IEC 24027:2020, 7.3.7"@en ;
    rdfs:comment "Simpson's paradox manifests when a trend that is indicated in individual groups of data reverses when the groups of data are combined."@en ;
    rdfs:label "Simpson's paradox"@en .

:ConfoundingVariableBias rdf:type :DataBias ;
    terms:source "ISO/IEC 24027:2020, 7.3.8"@en ;
    rdfs:coment "A confounding variable that influences both the dependent variable and independent variable causing a spurious association."@en ;
    rdfs:label "confounding variables"@en .

:NonNormality rdf:type :DataBias ;
    terms:source "ISO/IEC 24027:2020, 7.3.9"@en ;
    rdfs:comment "if the data is subject to a different distribution [from normal] (e.g. Chi-Square, Beta, Lorentz, Cauchy, Weibull or Pareto) the result might be biased and misleading."@en ;
    rdfs:label "non-normality"@en .

:OutlierNoiseBias rdf:type :DataBias ;
    terms:source "ISO/IEC 24027:2020, 7.3.10"@en ;
    rdfs:comment "Outliers are extreme data values that, if real, represent very low probability events of the to-be-modelled data. Noise is distortion which is characterised by a statistically-distributed variation of a physical quantity."@en ;
    rdfs:label "outliers and noise"@en .

:DataAggregationBias rdf:type :DataBias ;
    terms:source "ISO/IEC 24027:2020, 7.3.11; http://arxiv.org/abs/1901.10002"@en ;
    rdfs:comment "Aggregating data covering different groups of objects that might have different statistical distributions can introduce bias into the data used to train AI systems"@en ;
    rdfs:label "data aggregation bias"@en .

:DistributedTrainingBias rdf:type :DataBias ;
    terms:source "ISO/IEC 24027:2020, 7.3.12"@en ;
    rdfs:comment "Distributed ML might introduce its own cause for data bias as the different sources of data might not have the same distribution of feature space."@en ;
    rdfs:label "distributed training bias"@en .

:GroupAttributionBias rdf:type :CognitiveBias ;
    terms:source "ISO/IEC 24027:2020, 7.2.3"@en ;
    rdfs:comment "Group attribution bias occurs when a human assumes that what is true for an individual or object is also true for everyone, or all objects, in that group."@en ;
    rdfs:label "group attribution bias"@en .

:ImplicitBias rdf:type :CognitiveBias ;
    terms:source "ISO/IEC 24027:2020, 7.2.4"@en ;
    rdfs:comment "Implicit bias occurs when a human makes an association or assumption based on their mental models and memories."@en ;
    rdfs:label "implicit bias"@en .

:InGroupBias rdf:type :CognitiveBias ;
    terms:source "ISO/IEC 24027:2020, 7.2.6"@en ;
    rdfs:comment "In-group bias occurs when showing partiality to one's own group or own characteristics."@en ;
    rdfs:label "in-group bias"@en .

:OutGroupHomogeneityBias rdf:type :CognitiveBias ;
    terms:source "ISO/IEC 24027:2020, 7.2.7"@en ;
    rdfs:comment "Out-group homogeneity bias occurs when seeing out-group members as more alike than in-group members when comparing attitudes, values, personality traits, and other characteristics."@en ;
    rdfs:label "out-group homogeneity bias"@en .

:WYSIATIBias rdf:type :CognitiveBias ;
    terms:source "ISO IEC 24027:2020, 7.2.8 / https://www.microsoft.com/en-us/research/uploads/prod/2020/05/Fairlearn_WhitePaper-2020-09-22.pdf"@en ;
    rdfs:comment "'What You See Is All There Is' (WYSIATI) bias occurs when a human looks for information that confirms their beliefs, overlooks contradicting information, and draws conclusions based on what is familiar."@en ;
    rdfs:label "What you see is all there is bias"@en .

################################################################################
# Bias audits, a type of Documentation which must have an ML Model as domain
################################################################################
# Implicitly in being a subclass of airo:Documentation, ANY airo:AIComponent can have a bias audit on it
:BiasAudit rdf:type owl:Class ;
    rdfs:subClassOf airo:Documentation ;
    rdfs:comment "An audit which focuses on measuring bias in the AI system"@en ;
    rdfs:label "Bias audit"@en .
# :hasAudit property no longer required; use airo:hasDocumentation with a :BiasAudit.

# Very important to store the date that the audit was conducted
:auditDate rdf:type owl:ObjectProperty ;
    rdfs:domain :BiasAudit ;
    rdfs:range xsd:date ;
    rdfs:comment "Indicates the date that a bias audit was conducted"@en ;
    rdfs:label "Bias audit date" .

:BiasAudit rdfs:subClassOf [
    rdf:type owl:Restriction ;
    owl:onProperty :auditDate ;
    owl:cardinality "1"^^xsd:integer
] .

# A particular bias assertion should consist of:
#   1. A description of the groups involved in the test, and the reason for this test.
#   2. Indication of the fairness metric used for the test.
#   3. Indication of the test result (e.g., a float value)
#   4. Indication of the threshold for passing / failure, justifying what this threshold is supposed to represent.
#   5. Indication of whether the test passed or failed.
#   6. Indication of biases implied by this test.

:BiasAssertion rdf:type owl:Class ;
    rdfs:subClassOf earl:Assertion ;
    rdfs:comment "Indicates that an assertion measures bias"@en ;
    rdfs:label "Bias assertion"@en .

# Constraint to ensure any :BiasAssertion has a :Bias test subject
:BiasAssertion rdfs:subClassOf [
    rdf:type owl:Restriction ;
    owl:onProperty :testsBias ;
    owl:cardinality "1"^^xsd:nonNegativeInteger
] ,
[
    rdf:type owl:Restriction ;
    owl:onProperty :groupDescription ;
    owl:cardinality "1"^^xsd:nonNegativeInteger
] ,
[
    rdf:type owl:Restriction ;
    owl:onProperty :testThreshold ;
    owl:cardinality "1"^^xsd:nonNegativeInteger
] .

:BiasAssertion rdfs:subClassOf [
    rdf:type owl:Restriction ;
    owl:onProperty :hasFairnessMetric ;
    owl:cardinality "1"^^xsd:nonNegativeInteger
] .

# A custom 'tests bias' type. Purpose: Simplifies documentation.
# Avoids constructing specific conditions as in earl:TestCriterion ;
# 'Pass' when the bias tested for is deemed present, 'fail' when the bias tested for is deemed not present.
:testsBias rdf:type owl:ObjectProperty ;
    rdfs:domain :BiasAssertion ;
    rdfs:range :Bias ;
    rdfs:comment "Connects an Assertion with the bias type it is testing for."@en ;
    rdfs:label "Tests bias"@en .

:hasAssertion rdf:type owl:ObjectProperty ;
    rdfs:domain :BiasAudit ;
    rdfs:range earl:Assertion ;
    rdfs:comment "Connects a bias audit with an assertion"@en ;
    rdfs:label "has assertion"@en .

# A URI pointing to where the results reside
:testResultURI rdf:type owl:ObjectProperty ;
    rdfs:domain :BiasAssertion ;
    rdfs:range xsd:anyURI ;
    rdfs:comment "URI pointing to the test result (e.g., GitHub link)."@en ;
    rdfs:label "Result URI" .

# Description of the groups being tested in a bias assertion
:groupDescription rdf:type owl:ObjectProperty ;
    rdfs:domain :BiasAssertion ;
    rdfs:range xsd:string ;
    rdfs:comment "Provides a description of the groups which are compared in a bias assertion"@en ;
    rdfs:label "Group description"@en .

# Test thresholds
:Threshold rdf:type owl:Class ;
    rdfs:comment "A threshold associated with a bias test"@en ;
    rdfs:label "Threshold"@en .

:testThreshold rdf:type owl:ObjectProperty ;
    rdfs:domain :BiasAssertion ;
    rdfs:range :Threshold;
    rdfs:comment "Indicates the threshold associated with a particular bias test assertion"@en ;
    rdfs:label "test threshold"@en .

:ThresholdRange rdf:type owl:Class ;
    rdfs:subClassOf :Threshold ;
    rdfs:comment "A threshold which indicates a range of acceptable or unacceptable values"@en ;
    rdfs:label "Threshold range"@en .

:ThresholdBinary rdf:type owl:Class ;
    rdfs:subClassOf :Threshold ;
    rdfs:comment "A threshold which indicates a value, above or below which a test may be considered to have passed or failed"@en ;
    rdfs:label "Threshold binary"@en .

:thresholdBegin rdf:type owl:ObjectProperty ;
    rdfs:domain :ThresholdRange ;
    rdfs:range xsd:float , xsd:integer ;
    rdfs:comment "Indicates a float or integer beginning value for a range threshold"@en ;
    rdfs:label "threshold begin"@en .

:thresholdEnd rdf:type owl:ObjectProperty ;
    rdfs:domain :ThresholdRange ;
    rdfs:range xsd:float , xsd:integer ;
    rdfs:comment "Indicates a float or integer ending value for a range threshold"@en ;
    rdfs:label "threshold end"@en .

:binaryThreshold rdf:type owl:ObjectProperty ;
    rdfs:domain :ThresholdBinary ;
    rdfs:range xsd:float , xsd:integer ;
    rdfs:comment "Indicates a float or integer value for the binary threshold"@en ;
    rdfs:label "binary threshold"@en .

# OWL constraints on threshold objects
:ThresholdRange rdfs:subClassOf [
    rdf:type owl:Restriction ;
    owl:onProperty :thresholdBegin ;
    owl:cardinality "1"^^xsd:nonNegativeInteger
] ,
[
    rdf:type owl:Restriction ;
    owl:onProperty :thresholdEnd ;
    owl:cardinality "1"^^xsd:nonNegativeInteger
] .

:ThresholdBinary rdfs:subClassOf [
    rdf:type owl:Restriction ;
    owl:onProperty :binaryThreshold ;
    owl:cardinality "1"^^xsd:nonNegativeInteger
] .
# Test pass or fail indicates the nature of the thresholds

# Expand EARL to allow for numerical test results (not only pass / fail)
:FloatPass rdf:type owl:Class ;
    rdfs:subClassOf earl:Pass ;
    rdfs:comment "Indicates that a test results in a pass, with a floating point test result."@en ;
    rdfs:label "Float pass"@en .

:FloatFail rdf:type owl:Class ;
    rdfs:subClassOf earl:Fail ;
    rdfs:comment "Indicates that a test results in a fail, with a floating point test result."@en ;
    rdfs:label "Float fail"@en .

:IntegerPass rdf:type owl:Class ;
    rdfs:subClassOf earl:Pass ;
    rdfs:comment "Indicates that a test results in a pass, with an integer test result."@en ;
    rdfs:label "Integer pass"@en .

:IntegerFail rdf:type owl:Class ;
    rdfs:subClassOf earl:Fail ;
    rdfs:comment "Indicates that a test results in a fail, with an integer test result."@en ;
    rdfs:label "Integer fail"@en .

:floatValue rdf:type owl:ObjectProperty ;
    rdfs:domain :FloatPass , :FloatFail ;
    rdfs:range xsd:float ;
    rdfs:comment "Indicates the float value result associated with a FloatPass or FloatFail test result."@en ;
    rdfs:label "float value"@en .

:integerValue rdf:type owl:ObjectProperty ;
    rdfs:domain :IntegerPass , :IntegerFail ;
    rdfs:range xsd:integer ;
    rdfs:comment "Indicates the integer value result associated with an IntegerPass or IntegerFail test result."@en ;
    rdfs:label "integer value"@en .

# Enforce cardinality constraints for properties
:FloatPass rdfs:subClassOf [
    rdf:type owl:Restriction ;
    owl:onProperty :floatValue ;
    owl:cardinality "1"^^xsd:nonNegativeInteger
] .

:FloatFail rdfs:subClassOf [
    rdf:type owl:Restriction ;
    owl:onProperty :floatValue ;
    owl:cardinality "1"^^xsd:nonNegativeInteger
] .

:IntegerPass rdfs:subClassOf [
    rdf:type owl:Restriction ;
    owl:onProperty :integerValue ;
    owl:cardinality "1"^^xsd:nonNegativeInteger
] .

:IntegerFail rdfs:subClassOf [
    rdf:type owl:Restriction ;
    owl:onProperty :integerValue ;
    owl:cardinality "1"^^xsd:nonNegativeInteger
] .

# Add possibility to describe bias metrics.
:FairnessMetric rdf:type owl:Class ;
    terms:source "IBM AI Fairness 360 Glossary, https://aif360.res.ibm.com/resources#glossary"@en ;
    rdfs:comment "A quantification of unwanted bias in training data or models"@en ;
    rdfs:label "Fairness metric"@en .

:hasFairnessMetric rdf:type owl:ObjectProperty ;
    rdfs:domain :BiasAssertion ;
    rdfs:range :FairnessMetric ;
    rdfs:comment "Indicates that a test uses a particular fairness metric."@en ;
    rdfs:label "has fairness metric"@en .

# Fairness metrics from IBM AIF360
:StatisticalParityDifference rdf:type :FairnessMetric ;
    terms:source "IBM Cloud Pak for Data Docs, https://dataplatform.cloud.ibm.com/docs/content/wsj/model/wos-stat-parity-diff.html?context=cpdaas"@en ;
    rdfs:comment "The Statistical parity difference metric calculates the difference in the ratio of favorable outcomes between monitored groups and reference groups"@en ;
    rdfs:label "Statistical parity difference"@en .

:DisparateImpact rdf:type :FairnessMetric ;
    terms:source "IBM Cloud Pak for Data Docs, https://dataplatform.cloud.ibm.com/docs/content/wsj/model/wos-disparate-impact.html?context=analytic"@en ;
    rdfs:comment "Disparate impact compares the percentage of favorable outcomes for a monitored group to the percentage of favorable outcomes for a reference group"@en ;
    rdfs:label "Disparate impact"@en .

:EqualOpportunityDifference rdf:type :FairnessMetric ;
    terms:source "IBM AIF360 Web Page, https://aif360.res.ibm.com/"@en ;
    rdfs:comment "The difference of true positive rates between the unprivileged and the privileged groups"@en ;
    rdfs:label "Equal opportunity difference"@en .

:AverageOddsDifference rdf:type :FairnessMetric ;
    terms:source "IBM Cloud Pak for Data Docs, https://dataplatform.cloud.ibm.com/docs/content/wsj/model/wos-fairness-metrics-ovr.html?context=cpdaas"@en ;
    rdfs:comment "The average odds difference gives the percentage of transactions that was incorrectly scored by your model"@en ;
    rdfs:label "Average odds difference"@en .

:AverageAbsOddsDifference rdf:type :FairnessMetric ;
    terms:source "IBM Cloud Pak for Data Docs, https://dataplatform.cloud.ibm.com/docs/content/wsj/model/wos-fairness-metrics-ovr.html?context=cpdaas"@en ;
    rdfs:comment "The average absolute odds difference compares the average of absolute difference in false positive rates and true positive rates between monitored groups and reference groups"@en ;
    rdfs:label "Average absolute odds difference"@en .

:ErrorRateDifference rdf:type :FairnessMetric ;
    terms:source "IBM Cloud Pak for Data Docs, https://dataplatform.cloud.ibm.com/docs/content/wsj/model/wos-fairness-metrics-ovr.html?context=cpdaas"@en ;
    rdfs:comment "The error rate difference calculates the percentage of transactions that are incorrectly scored by your model"@en ;
    rdfs:label "Error rate difference"@en .

:ErrorRateRatio rdf:type :FairnessMetric ;
    terms:source "IBM AIF360 Python Docs, https://aif360.readthedocs.io/en/stable/modules/generated/aif360.metrics.ClassificationMetric.html#aif360.metrics.ClassificationMetric"@en ;
    rdfs:comment "(False positives + False negatives) divided by (Positives + Negatives) "@en ;    # (FP+FN)/(P+N)
    rdfs:label "Error rate ratio"@en .

:FalseDiscoveryRateDifference rdf:type :FairnessMetric ;
    terms:source "IBM Cloud Pak for Data Docs, https://dataplatform.cloud.ibm.com/docs/content/wsj/model/wos-fairness-metrics-ovr.html?context=cpdaas"@en ;
    rdfs:comment "The false discovery rate difference gives the amount of false positive transactions as a percentage of all transactions with a positive outcome"@en ;
    rdfs:label "False discovery rate difference"@en .

:FalseDiscoveryRateRatio rdf:type :FairnessMetric ;
    terms:source "IBM AIF360 Python Docs, https://aif360.readthedocs.io/en/stable/modules/generated/aif360.metrics.ClassificationMetric.html#aif360.metrics.ClassificationMetric"@en ;
    rdfs:comment "(False discovery rate for unprivileged group) divided by (False discovery rate for privileged group)"@en ; # FDRu/FDRp
    rdfs:label "False discovery rate ratio"@en .

:FalseNegativeRateRatio rdf:type :FairnessMetric ;
    terms:source "IBM AIF360 Python Docs, https://aif360.readthedocs.io/en/stable/modules/generated/aif360.metrics.ClassificationMetric.html#aif360.metrics.ClassificationMetric"@en ;
    rdfs:comment "(False negative rate for the unprivileged group) divided by (False negative rate for the privileged group)"@en ; # FNRu/FNRp
    rdfs:label "False negative rate ratio"@en .

:FalseOmissionRateDifference rdf:type :FairnessMetric ;
    terms:source "IBM Cloud Pak for Data Docs, https://dataplatform.cloud.ibm.com/docs/content/wsj/model/wos-fairness-metrics-ovr.html?context=cpdaas"@en ;
    rdfs:comment "The false omission rate difference gives the number of false negative transactions as a percentage of all transactions with a negative outcome"@en ;
    rdfs:label "False omission rate difference"@en .

:FalseOmissionRateRatio rdf:type :FairnessMetric ;
    terms:source "IBM AIF360 Python Docs, https://aif360.readthedocs.io/en/stable/modules/generated/aif360.metrics.ClassificationMetric.html#aif360.metrics.ClassificationMetric"@en ;
    rdfs:comment "(False omission rate for unprivileged group) divided by (False omission rate for privileged group)"@en ; # FORu/FORp
    rdfs:label "False omission rate ratio"@en .

:FalsePositiveRateRatio rdf:type :FairnessMetric ;
    terms:source "IBM AIF360 Python Docs, https://aif360.readthedocs.io/en/stable/modules/generated/aif360.metrics.ClassificationMetric.html#aif360.metrics.ClassificationMetric" ;
    rdfs:comment "(False positive rate for unprivileged group) divided by (False positive rate for privileged group)"@en ;
    rdfs:label "False positive rate ratio"@en .

:FalseNegativeRateDifference rdf:type :FairnessMetric ;
    terms:source "IBM AIF360 Python Docs, https://aif360.readthedocs.io/en/stable/modules/generated/aif360.metrics.ClassificationMetric.html#aif360.metrics.ClassificationMetric" ;
    rdfs:comment "(False negative rate for unprivileged group) divided by (False negative rate for privileged group)"@en ; # FNRu-FNRp
    rdfs:label "False negative rate difference"@en .

:FalsePositiveRateDifference rdf:type :FairnessMetric ;
    terms:source "IBM AIF360 Python Docs, https://aif360.readthedocs.io/en/stable/modules/generated/aif360.metrics.ClassificationMetric.html#aif360.metrics.ClassificationMetric" ;
    rdfs:comment "(False positive rate for unprivileged group) minus (False positive rate for privileged group)"@en ;   # FPRu-FPRp
    rdfs:label "False positive rate difference"@en .

:TruePositiveRateDifference rdf:type :FairnessMetric ;
    terms:source "IBM AIF360 Python Docs, https://aif360.readthedocs.io/en/stable/modules/generated/aif360.metrics.ClassificationMetric.html#aif360.metrics.ClassificationMetric" ;
    rdfs:comment "The ratio of true positives to positive examples in the dataset, TPR = TP/P"@en ;
    rdfs:label "True positive rate difference"@en .

:CoefficientOfVariation rdf:type :FairnessMetric ;
    terms:source "IBM AIF360 Python Docs, https://aif360.readthedocs.io/en/stable/modules/generated/aif360.metrics.ClassificationMetric.html#aif360.metrics.ClassificationMetric" ;
    rdfs:comment "The square root of two times the generalize entropy index"@en ;
    rdfs:label "Coefficient of variation"@en .

:TheilIndex rdf:type :FairnessMetric ;
    terms:source "IBM AIF360 Python Docs, https://aif360.readthedocs.io/en/stable/modules/generated/aif360.metrics.ClassificationMetric.html#aif360.metrics.ClassificationMetric" ;
    rdfs:comment "The Theil index is the generalized entropy index with alpha = 1" ;
    rdfs:label "Theil index"@en .

:BetweenGroupTheilIndex rdf:type :FairnessMetric ;
    terms:source "IBM AIF360 Python Docs, https://aif360.readthedocs.io/en/stable/modules/generated/aif360.metrics.ClassificationMetric.html#aif360.metrics.ClassificationMetric" ;
    rdfs:comment "The between group generalized entropy index with alpha = 1"@en ;
    rdfs:label "Between group Theil index"@en .

:BetweenGroupCoefficientOfVariation rdf:type :FairnessMetric ;
    terms:source "IBM AIF360 Python Docs, https://aif360.readthedocs.io/en/stable/modules/generated/aif360.metrics.ClassificationMetric.html#aif360.metrics.ClassificationMetric" ;
    rdfs:comment "The square root of two times the between group generalized entropy index with alpha = 2"@en ;
    rdfs:label "Between group coefficient of variation"@en .

:BetweenAllGroupsCoefficientOfVariation rdf:type :FairnessMetric ;
    terms:source "IBM AIF360 Python Docs, https://aif360.readthedocs.io/en/stable/modules/generated/aif360.metrics.ClassificationMetric.html#aif360.metrics.ClassificationMetric" ;
    rdfs:comment "The square root of two times the between all groups generalized entropy index with alpha = 2"@en ;
    rdfs:label "Between all groups coefficient of variation"@en .

:BetweenAllGroupsGeneralisedEntropyIndex rdf:type :FairnessMetric ;
    terms:source "IBM AIF360 Python Docs, https://aif360.readthedocs.io/en/stable/modules/generated/aif360.metrics.ClassificationMetric.html#aif360.metrics.ClassificationMetric" ;
    rdfs:comment "Between-group generalized entropy index that uses all combinations of groups based on self.dataset.protected_attributes"@en ;
    rdfs:label "Between all groups generalised entropy index"@en .

:ConsistencyMetric rdf:type :FairnessMetric ;
    terms:source "IBM AIF360 Docs, https://aif360.readthedocs.io/en/stable/modules/generated/aif360.metrics.ClassificationMetric.html#aif360.metrics.ClassificationMetric" ;
    rdfs:comment "Individual fairness metric that measures how similar the labels are for similar instances"@en ;
    rdfs:label "Consistency metric"@en .

:GeneralisedEntropyIndex rdf:type :FairnessMetric ;
    terms:source "A Unified Approach to Quantifying Algorithmic Unfairness: Measuring Individual & Group Unfairness via Inequality Indices. https://arxiv.org/abs/1807.00787" ;
    rdfs:comment "Generalized entropy index is a measure of unfairness which can be interpreted as a measure of information theoretic redundancy in data."@en ;
    rdfs:label "Generalised entropy index"@en .

:BetweenGroupGeneralisedEntropyIndex rdf:type :FairnessMetric ;
    terms:source "IBM AIF360 Python Docs, https://aif360.readthedocs.io/en/stable/modules/generated/aif360.metrics.ClassificationMetric.html#aif360.metrics.ClassificationMetric" ;
    rdfs:comment "Between-group generalized entropy index that uses self.privileged_groups and self.unprivileged_groups as the only two groups"@en ;
    rdfs:label "Between groups generalised entropy index"@en .

:MeanEuclideanDistanceDifference rdf:type :FairnessMetric ;
    terms:source "IBM AIF360 Python Docs, https://aif360.readthedocs.io/en/stable/modules/generated/aif360.metrics.SampleDistortionMetric.html#aif360.metrics.SampleDistortionMetric"@en ;
    rdfs:comment "Difference of the average Euclidean distances"@en ;
    rdfs:label "Mean Euclidean distance difference"@en .

:MeanEuclideanDistanceRatio rdf:type :FairnessMetric ;
    terms:source "IBM AIF360 Python Docs, https://aif360.readthedocs.io/en/stable/modules/generated/aif360.metrics.SampleDistortionMetric.html#aif360.metrics.SampleDistortionMetric"@en ;
    rdfs:comment "Ratio of the average Euclidean distances"@en ;
    rdfs:label "Mean Euclidean distance ratio"@en .

:MeanMahalanobisDistanceDifference rdf:type :FairnessMetric ;
    terms:source "IBM AIF360 Python Docs, https://aif360.readthedocs.io/en/stable/modules/generated/aif360.metrics.SampleDistortionMetric.html#aif360.metrics.SampleDistortionMetric"@en ;
    rdfs:comment "Difference of the average Mahalanobis distances"@en ;
    rdfs:label "Mean Mahalanobis distance difference"@en .

:MeanMahalanobisDistanceRatio rdf:type :FairnessMetric ;
    terms:source "IBM AIF360 Python Docs, https://aif360.readthedocs.io/en/stable/modules/generated/aif360.metrics.SampleDistortionMetric.html#aif360.metrics.SampleDistortionMetric"@en ;
    rdfs:comment "Ratio of the average Mahalanobis distances"@en ;
    rdfs:label "Mean Mahalanobis distance ratio"@en .

:MeanManhattanDistanceDifference rdf:type :FairnessMetric ;
    terms:source "IBM AIF360 Python Docs, https://aif360.readthedocs.io/en/stable/modules/generated/aif360.metrics.SampleDistortionMetric.html#aif360.metrics.SampleDistortionMetric"@en ;
    rdfs:comment "Difference of the average Manhattan distances"@en ;
    rdfs:label "Mean Manhattan distance difference"@en .

:MeanManhattanDistanceRatio rdf:type :FairnessMetric ;
    terms:source "IBM AIF360 Python Docs, https://aif360.readthedocs.io/en/stable/modules/generated/aif360.metrics.SampleDistortionMetric.html#aif360.metrics.SampleDistortionMetric"@en ;
    rdfs:comment "Ratio of the average Manhattan distances"@en ;
    rdfs:label "Mean Manhattan distance ratio"@en .

:BaseRateMetric rdf:type :FairnessMetric ;
    terms:source "IBM AIF360 Python Docs, https://aif360.readthedocs.io/en/stable/modules/generated/aif360.metrics.BinaryLabelDatasetMetric.html#aif360.metrics.BinaryLabelDatasetMetric"@en ;
    rdfs:comment "Pr(Y=1) = P/(P+N)"@en ;
    rdfs:label "Base rate metric"@en .

:SmoothedEmpiricalDifferentialFairness rdf:type :FairnessMetric ;
    terms:source "IBM AIF360 Python Docs, https://aif360.readthedocs.io/en/stable/modules/generated/aif360.metrics.BinaryLabelDatasetMetric.html#aif360.metrics.BinaryLabelDatasetMetric"@en ;
    rdfs:comment "Smoothed empirical differential fairness"@en ;
    rdfs:label "Smoothed empirical differential fairness"@en .

:RichSubgroupMetric rdf:type :FairnessMetric ;
    terms:source "IBM AIF360 Python Docs, https://aif360.readthedocs.io/en/stable/modules/generated/aif360.metrics.BinaryLabelDatasetMetric.html#aif360.metrics.BinaryLabelDatasetMetric"@en ;
    rdfs:comment "Audit dataset with respect to rich subgroups defined by linear thresholds of sensitive attributes"@en ;
    rdfs:label "Rich subgroup metric"@en .

:DifferentialFairnessBiasAmplification rdf:type :FairnessMetric ;
    terms:source "IBM AIF360 Python Docs, https://aif360.readthedocs.io/en/stable/modules/generated/aif360.metrics.MDSSClassificationMetric.html#aif360.metrics.MDSSClassificationMetric"@en ;
    rdfs:comment "Bias amplification is the difference in smoothed EDF between the classifier and the original dataset"@en ;
    rdfs:label "Differential fairness bias amplification"@en .

:MDSSBiasScore rdf:type :FairnessMetric ;   # from score_groups of MDSSClassificationMetric
    terms:source "IBM AIF360 Python Docs, https://aif360.readthedocs.io/en/stable/modules/generated/aif360.metrics.MDSSClassificationMetric.html#aif360.metrics.MDSSClassificationMetric"@en ;
    rdfs:comment "The bias score for a prespecified group of records"@en ;
    rdfs:label "MDSS bias score"@en .

# Mitigation applied on tests
:mitigationApplied rdf:type owl:ObjectProperty ;
    rdfs:domain :BiasAssertion , :BiasAudit ;
    rdfs:range :BiasMitigationMeasure ;
    rdfs:comment "Indicates a mitigation measure applied to a bias assertion"@en ;
    rdfs:label "Mitigation applied"@en .

:BiasMitigationMeasure rdf:type owl:Class ;
    rdfs:subClassOf airo:Control ;
    rdfs:comment "A mitigation measure for bias"@en ;
    rdfs:label "Bias mitigation measure"@en .

# Bias mitigation metrics in IBM AI fairness 360
:OptimizedPreprocessing rdf:type :BiasMitigationMeasure ;
    terms:source "IBM AIF360 Python Docs, https://aif360.readthedocs.io/en/stable/modules/algorithms.html"@en ;
    rdfs:comment "A preprocessing technique that learns a probabilistic transformation that edits the features and labels in the data with group fairness, individual distortion, and data fidelity constraints and objectives."@en ;
    rdfs:label "Optimized preprocessing"@en .

:DisparateImpactRemover rdf:type :BiasMitigationMeasure ;
    terms:source "IBM AIF360 Python Docs, https://aif360.readthedocs.io/en/stable/modules/algorithms.html"@en ;
    rdfs:comment "Disparate impact remover is a preprocessing technique that edits feature values increase group fairness while preserving rank-ordering within groups."@en ;
    rdfs:label "Disparate impact remover"@en .

:EqualizedOddsPostprocessing rdf:type :BiasMitigationMeasure ;
    terms:source "IBM AIF360 Python Docs, https://aif360.readthedocs.io/en/stable/modules/algorithms.html"@en ;
    rdfs:comment "A post-processing technique that solves a linear program to find probabilities with which to change output labels to optimize equalized odds."@en ;
    rdfs:label "Equalized odds postprocessing"@en .

:Reweighing rdf:type :BiasMitigationMeasure ;
    terms:source "IBM AIF360 Python Docs, https://aif360.readthedocs.io/en/stable/modules/algorithms.html"@en ;
    rdfs:comment "Reweighing is a preprocessing technique that Weights the examples in each (group, label) combination differently to ensure fairness before classification."@en ;
    rdfs:label "Reweighing"@en .

:RejectOptionClassification rdf:type :BiasMitigationMeasure ;
    terms:source "IBM AIF360 Python Docs, https://aif360.readthedocs.io/en/stable/modules/algorithms.html"@en ;
    rdfs:comment "Reject option classification is a postprocessing technique that gives favorable outcomes to unprivileged groups and unfavorable outcomes privileged groups in a confidence band around the decision boundary with the highest uncertainty."@en ;
    rdfs:label "Reject option classification"@en .

:PrejudiceRemoverRegularizer rdf:type :BiasMitigationMeasure ;
    terms:source "IBM AIF360 Python Docs, https://aif360.readthedocs.io/en/stable/modules/algorithms.html"@en ;
    rdfs:comment "Prejudice remover is an in-processing technique that adds a discrimination-aware regularization terms to the learning objective."@en ;
    rdfs:label "Prejudice remover regularizer"@en .

:CalibratedEqualizedOddsPostprocessing rdf:type :BiasMitigationMeasure ;
    terms:source "IBM AIF360 Python Docs, https://aif360.readthedocs.io/en/stable/modules/algorithms.html"@en ;
    rdfs:comment "Calibrated equalized odds postprocessing is a post-processing technique that optimizes over calibrated classifier score outputs to find probabilities with which to change output labels with an equalized odds objective."@en ;
    rdfs:label "Calibrated equalized odds postprocessing"@en .

:LearningFairRepresentations rdf:type :BiasMitigationMeasure ;
    terms:source "IBM AIF360 Python Docs, https://aif360.readthedocs.io/en/stable/modules/algorithms.html"@en ;
    rdfs:comment "Learning fair representations is a pre-processing technique that finds a latent representation which encodes the data well but obfuscates information about protected attributes."@en ;
    rdfs:label "Learning fair representations"@en .

:AdversarialDebiasing rdf:type :BiasMitigationMeasure ;
    terms:source "IBM AIF360 Python Docs, https://aif360.readthedocs.io/en/stable/modules/algorithms.html"@en ;
    rdfs:comment "Adversarial debiasing is an in-processing technique that learns a classifier to maximize prediction accuracy and simultaneously reduce an adversary's ability to determine the protected attribute from the predictions."@en ;
    rdfs:label "Adversarial debiasing"@en .

:MetaAlgorithmFairClassification rdf:type :BiasMitigationMeasure ;
    terms:source "IBM AIF360 Python Docs, https://aif360.readthedocs.io/en/stable/modules/algorithms.html"@en ;
    rdfs:comment "The meta algorithm here takes the fairness metric as part of the input and returns a classifier optimized w.r.t."@en ;
    rdfs:label "Meta algorithm fair classification"@en .

:RichSubgroupFairness rdf:type :BiasMitigationMeasure ;
    terms:source "IBM AIF360 Python Docs, https://aif360.readthedocs.io/en/stable/modules/algorithms.html"@en ;
    rdfs:comment "Model is an algorithm for learning classifiers that are fair with respect to rich subgroups"@en ;
    rdfs:label "Rich subgroup fairness"@en .

:ExponentiatedGradientReduction rdf:type :BiasMitigationMeasure ;
    terms:source "IBM AIF360 Python Docs, https://aif360.readthedocs.io/en/stable/modules/algorithms.html"@en ;
    rdfs:comment "Exponentiated gradient reduction for fair classification"@en ;
    rdfs:label "Exponentiated gradient reduction"@en .

:GridSearchReduction rdf:type :BiasMitigationMeasure ;
    terms:source "IBM AIF360 Python Docs, https://aif360.readthedocs.io/en/stable/modules/algorithms.html"@en ;
    rdfs:comment "Grid search reduction for fair classification or regression"@en ;
    rdfs:label "Grid search reduction"@en .

# Expand with AIO categories --- should the AIO namespace be used?
:ComputationalBias rdf:type owl:Class ;
    terms:source "https://bioportal.bioontology.org/ontologies/AIO/?p=classes&conceptid=root"@en ;
    rdfs:comment "A systematic tendency which causes differences between results and facts. The bias exists in numbers of the process of data analysis, including the source of the data, the estimator chosen, and the ways the data was analyzed."@en ;
    rdfs:label "computational bias"@en ;
    rdfs:subClassOf :Bias .

:ProcessingBias rdf:type owl:Class ;
    terms:source "https://bioportal.bioontology.org/ontologies/AIO/?p=classes&conceptid=https%3A%2F%2Fw3id.org%2Faio%2FProcessingBias"@en ;
    rdfs:comment "Judgement modulated by affect, which is influenced by the level of efficacy and efficiency in information processing; in cognitive sciences, processing bias is often referred to as an aesthetic judgement."@en ;
    rdfs:label "processing bias"@en ;
    rdfs:subClassOf :ComputationalBias .

:AmplificationBias rdf:type owl:Class ;
    terms:source "https://bioportal.bioontology.org/ontologies/AIO/?p=classes&conceptid=https%3A%2F%2Fw3id.org%2Faio%2FAmplificationBias"@en ;
    rdfs:comment "Arises when the distribution over prediction outputs is skewed in comparison to the prior distribution of the prediction target"@en ;
    rdfs:label "amplification bias"@en ;
    rdfs:subClassOf :ProcessingBias .

:ErrorPropagationBias rdf:type owl:Class ;
    terms:source "https://bioportal.bioontology.org/ontologies/AIO/?p=classes&conceptid=https%3A%2F%2Fw3id.org%2Faio%2FErrorPropagationBias"@en ;
    rdfs:comment "The effect of variables' uncertainties (or errors, more specifically random errors) on the uncertainty of a function based on them"@en ;
    rdfs:label "error propagation bias"@en ;
    rdfs:subClassOf :ProcessingBias .

:InheritedBias rdf:type owl:Class ;
    terms:source "https://bioportal.bioontology.org/ontologies/AIO/?p=classes&conceptid=https%3A%2F%2Fw3id.org%2Faio%2FInheritedBias"@en ;
    rdfs:comment "Arises when applications that are built with machine learning are used to generate inputs for other machine learning algorithms. If the output is biased in any way, this bias may be inherited by systems using the output as input to learn other models."@en ;
    rdfs:label "inherited bias"@en ;
    rdfs:subClassOf :ProcessingBias .

:ModelSelectionBias rdf:type owl:Class ;
    terms:source "https://bioportal.bioontology.org/ontologies/AIO/?p=classes&conceptid=https%3A%2F%2Fw3id.org%2Faio%2FModelSelectionBias"@en ;
    rdfs:comment "The bias introduced while using the data to select a single seemingly 'best' model from a large set of models employing many predictor variables. Model selection bias also occurs when an explanatory variable has a weak relationship with the response variable."@en ;
    rdfs:label "model selection bias"@en ;
    rdfs:subClassOf :ComputationalBias .

:SurvivorshipBias rdf:type owl:Class ;
    terms:source "https://bioportal.bioontology.org/ontologies/AIO/?p=classes&conceptid=https%3A%2F%2Fw3id.org%2Faio%2FSurvivorshipBias"@en ;
    rdfs:comment "Tendency for people to focus on the items, observations, or people that 'survive' or make it past a selection process, while overlooking those that did not."@en ;
    rdfs:label "survivorship bias"@en ;
    rdfs:subClassOf :ComputationalBias .

:SelectionAndSamplingBias rdf:type owl:Class ;
    terms:source "https://bioportal.bioontology.org/ontologies/AIO/?p=classes&conceptid=https%3A%2F%2Fw3id.org%2Faio%2FSelectionAndSamplingBias"@en ;
    rdfs:comment "Bias introduced by the selection of individuals, groups, or data for analysis in such a way that proper randomization is not achieved, thereby failing to ensure that the sample obtained is representative of the population intended to be analyzed."@en ;
    rdfs:label "selection and sampling bias"@en ;
    rdfs:subClassOf :DataBias .

:DataGenerationBias rdf:type owl:Class ;
    terms:source "https://bioportal.bioontology.org/ontologies/AIO/?p=classes&conceptid=https%3A%2F%2Fw3id.org%2Faio%2FDataGenerationBias"@en ;
    rdfs:comment "Arises from the addition of synthetic or redundant data samples to a dataset"@en ;
    rdfs:label "data generation bias"@en ;
    rdfs:subClassOf :DataBias .

:DetectionBias rdf:type owl:Class ;
    terms:source "https://bioportal.bioontology.org/ontologies/AIO/?p=classes&conceptid=https%3A%2F%2Fw3id.org%2Faio%2FDetectionBias"@en ;
    rdfs:comment "Systematic differences between groups in how outcomes are determined and may cause an over- or underestimation of the size of the effect."@en ;
    rdfs:label "detection bias"@en ;
    rdfs:subClassOf :DataBias .

:EcologicalFallacyBias rdf:type owl:Class ;
    terms:source "https://bioportal.bioontology.org/ontologies/AIO/?p=classes&conceptid=https%3A%2F%2Fw3id.org%2Faio%2FEcologicalFallacyBias"@en ;
    rdfs:comment "Occurs when an inference is made about an individual based on their membership within a group."@en ;
    rdfs:label "ecological fallacy bias"@en ;
    rdfs:subClassOf :DataBias .

:EvaluationBias rdf:type owl:Class ;
    terms:source "https://bioportal.bioontology.org/ontologies/AIO/?p=classes&conceptid=https%3A%2F%2Fw3id.org%2Faio%2FEvaluationBias"@en ;
    rdfs:comment "Arises when the testing or external benchmark populations do not equally represent the various parts of the user population or from the use of performance metrics that are not appropriate for the way in which the model will be used."@en ;
    rdfs:label "evaluation bias"@en ;
    rdfs:subClassOf :DataBias .

:ExclusionBias rdf:type owl:Class ;
    terms:source "https://bioportal.bioontology.org/ontologies/AIO/?p=classes&conceptid=https%3A%2F%2Fw3id.org%2Faio%2FExclusionBias"@en ;
    rdfs:comment "When specific groups of user populations are excluded from testing and subsequent analyses."@en ;
    rdfs:label "exclusion bias"@en ;
    rdfs:subClassOf :DataBias .

:MeasurementBias rdf:type owl:Class ;
    terms:source "https://bioportal.bioontology.org/ontologies/AIO/?p=classes&conceptid=https%3A%2F%2Fw3id.org%2Faio%2FMeasurementBias"@en ;
    rdfs:comment "Arises when features and labels are proxies for desired quantities, potentially leaving out important factors or introducing group or input-dependent noise that leads to differential performance."@en ;
    rdfs:label "measurement bias"@en ;
    rdfs:subClassOf :DataBias .

:PopularityBias rdf:type owl:Class ;
    terms:source "https://bioportal.bioontology.org/ontologies/AIO/?p=classes&conceptid=https%3A%2F%2Fw3id.org%2Faio%2FPopularityBias"@en ;
    rdfs:comment "A form of selection bias that occurs when items that are more popular are more exposed and less popular items are under-represented."@en ;
    rdfs:label "popularity bias"@en ;
    rdfs:subClassOf :DataBias .

:PopulationBias rdf:type owl:Class ;
    terms:source "https://bioportal.bioontology.org/ontologies/AIO/?p=classes&conceptid=https%3A%2F%2Fw3id.org%2Faio%2FPopulationBias"@en ;
    rdfs:comment "A form of selection bias that occurs when items that are more popular are more exposed and less popular items are under-represented.aSystematic distortions in demographics or other user characteristics between a population of users represented in a dataset or on a platform and some target population."@en ;
    rdfs:label "population bias"@en ;
    rdfs:subClassOf :DataBias .

:RepresentationBias rdf:type owl:Class ;
    terms:source "https://bioportal.bioontology.org/ontologies/AIO/?p=classes&conceptid=https%3A%2F%2Fw3id.org%2Faio%2FRepresentationBias"@en ;
    rdfs:comment "Arises due to non-random sampling of subgroups, causing trends estimated for one population to not be generalizable to data collected from a new population."@en ;
    rdfs:label "representation bias"@en ;
    rdfs:subClassOf :DataBias .

:TemporalBias rdf:type owl:Class ;
    terms:source "https://bioportal.bioontology.org/ontologies/AIO/?p=classes&conceptid=https%3A%2F%2Fw3id.org%2Faio%2FTemporalBias"@en ;
    rdfs:comment "Bias that arises from differences in populations and behaviors over time."@en ;
    rdfs:label "temporal bias"@en ;
    rdfs:subClassOf :DataBias .

:UncertaintyBias rdf:type owl:Class ;
    terms:source "https://bioportal.bioontology.org/ontologies/AIO/?p=classes&conceptid=https%3A%2F%2Fw3id.org%2Faio%2FUncertaintyBias"@en ;
    rdfs:comment "Arises when predictive algorithms favor groups that are better represented in the training data, since there will be less uncertainty associated with those predictions."@en ;
    rdfs:label "uncertainty bias"@en ;
    rdfs:subClassOf :DataBias .

:UseAndInterpretationBias rdf:type owl:Class ;
    terms:source "https://bioportal.bioontology.org/ontologies/AIO/?p=classes&conceptid=https%3A%2F%2Fw3id.org%2Faio%2FUseAndInterpretationBias"@en ;
    rdfs:comment "An information-processing bias, the tendency to inappropriately analyze ambiguous stimuli, scenarios and events."@en ;
    rdfs:label "use and interpretation bias"@en ;
    rdfs:subClassOf :Bias .

:ActivityBias rdf:type owl:Class ;
    terms:source "https://bioportal.bioontology.org/ontologies/AIO/?p=classes&conceptid=https%3A%2F%2Fw3id.org%2Faio%2FActivityBias"@en ;
    rdfs:comment "A type of selection bias that occurs when systems/platforms get their training data from their most active users, rather than those less active (or inactive)."@en ;
    rdfs:label "activity bias"@en ;
    rdfs:subClassOf :UseAndInterpretationBias .

:ConceptDriftBias rdf:type owl:Class ;
    terms:source "https://bioportal.bioontology.org/ontologies/AIO/?p=classes&conceptid=https%3A%2F%2Fw3id.org%2Faio%2FConceptDriftBias"@en ;
    rdfs:comment "Use of a system outside the planned domain of application, and a common cause of performance gaps between laboratory settings and the real world."@en ;
    rdfs:label "concept drift bias"@en ;
    rdfs:subClassOf :UseAndInterpretationBias .

:ContentProductionBias rdf:type owl:Class ;
    terms:source "https://bioportal.bioontology.org/ontologies/AIO/?p=classes&conceptid=https%3A%2F%2Fw3id.org%2Faio%2FContentProductionBias"@en ;
    rdfs:comment "Arises from structural, lexical, semantic, and syntactic differences in the contents generated by users."@en ;
    rdfs:label "content production bias"@en ;
    rdfs:subClassOf :UseAndInterpretationBias .

:DataDredgingBias rdf:type owl:Class ;
    terms:source "https://bioportal.bioontology.org/ontologies/AIO/?p=classes&conceptid=https%3A%2F%2Fw3id.org%2Faio%2FDataDredgingBias"@en ;
    rdfs:comment "A statistical bias in which testing huge numbers of hypotheses of a dataset may appear to yield statistical significance even when the results are statistically nonsignificant."@en ;
    rdfs:label "data dredging bias"@en ;
    rdfs:subClassOf :UseAndInterpretationBias .

:EmergentBias rdf:type owl:Class ;
    terms:source "https://bioportal.bioontology.org/ontologies/AIO/?p=classes&conceptid=https%3A%2F%2Fw3id.org%2Faio%2FEmergentBias"@en ;
    rdfs:comment "Emergent bias is the result of the use and reliance on algorithms across new or unanticipated contexts."@en ;
    rdfs:label "emergent bias"@en ;
    rdfs:subClassOf :UseAndInterpretationBias .

:FeedbackLoopBias rdf:type owl:Class ;
    terms:source "https://bioportal.bioontology.org/ontologies/AIO/?p=classes&conceptid=https%3A%2F%2Fw3id.org%2Faio%2FFeedbackLoopBias"@en ;
    rdfs:comment "Effects that may occur when an algorithm learns from user behavior and feeds that behavior back into the model."@en ;
    rdfs:label "feedback loop bias"@en ;
    rdfs:subClassOf :UseAndInterpretationBias .

:HostileAttributionBias rdf:type owl:Class ;
    terms:source "https://bioportal.bioontology.org/ontologies/AIO/?p=classes&conceptid=https%3A%2F%2Fw3id.org%2Faio%2FHostileAttributionBias"@en ;
    rdfs:comment "A bias wherein individuals perceive benign or ambiguous behaviors as hostile."@en ;
    rdfs:label "hostile attribution bias"@en ;
    rdfs:subClassOf :UseAndInterpretationBias .

:LinkingBias rdf:type owl:Class ;
    terms:source "https://bioportal.bioontology.org/ontologies/AIO/?p=classes&conceptid=https%3A%2F%2Fw3id.org%2Faio%2FLinkingBias"@en ;
    rdfs:comment "Arises when network attributes obtained from user connections, activities, or interactions differ and misrepresent the true behavior of the users."@en ;
    rdfs:label "linking bias"@en ;
    rdfs:subClassOf :UseAndInterpretationBias .

:GroupBias rdf:type owl:Class ;
    terms:source "https://bioportal.bioontology.org/ontologies/AIO/?p=classes&conceptid=https%3A%2F%2Fw3id.org%2Faio%2FGroupBias"@en ;
    rdfs:comment "A pattern of favoring members of one's in-group over out-group members. This can be expressed in evaluation of others, in allocation of resources, and in many other ways."@en ;
    rdfs:label "group bias"@en ;
    rdfs:subClassOf :CognitiveBias .

:DeploymentBias rdf:type owl:Class ;
    terms:source "https://bioportal.bioontology.org/ontologies/AIO/?p=classes&conceptid=https%3A%2F%2Fw3id.org%2Faio%2FDeploymentBias"@en ;
    rdfs:comment "Arises when systems are used as decision aids for humans, since the human intermediary may act on predictions in ways that are typically not modeled in the system. However, it is still individuals using the deployed system."@en ;
    rdfs:label "deployment bias"@en ;
    rdfs:subClassOf :GroupBias .

:FundingBias rdf:type owl:Class ;
    terms:source "https://bioportal.bioontology.org/ontologies/AIO/?p=classes&conceptid=https%3A%2F%2Fw3id.org%2Faio%2FFundingBias"@en ;
    rdfs:comment "Arises when biased results are reported in order to support or satisfy the funding agency or financial supporter of the research study, but it can also be the individual researcher."@en ;
    rdfs:label "funding bias"@en ;
    rdfs:subClassOf :GroupBias .

:GroupthinkBias rdf:type owl:Class ;
    terms:source "https://bioportal.bioontology.org/ontologies/AIO/?p=classes&conceptid=https%3A%2F%2Fw3id.org%2Faio%2FGroupthinkBias"@en ;
    rdfs:comment "A psychological phenomenon that occurs when people in a group tend to make non-optimal decisions based on their desire to conform to the group, or fear of dissenting with the group. In groupthink, individuals often refrain from expressing their personal disagreement with the group, hesitating to voice opinions that do not align with the group."@en ;
    rdfs:label "Groupthink bias"@en ;
    rdfs:subClassOf :GroupBias .

:IndividualBias rdf:type owl:Class ;
    terms:source "https://bioportal.bioontology.org/ontologies/AIO/?p=classes&conceptid=https%3A%2F%2Fw3id.org%2Faio%2FIndividualBias"@en ;
    rdfs:comment "Individual bias is a persistent point of view or limited list of such points of view that one applies ('parent', 'academic', 'professional', or etc.)."@en ;
    rdfs:label "individual bias"@en ;
    rdfs:subClassOf :CognitiveBias .

:AnchoringBias rdf:type owl:Class ;
    terms:source "https://bioportal.bioontology.org/ontologies/AIO/?p=classes&conceptid=https%3A%2F%2Fw3id.org%2Faio%2FAnchoringBias"@en ;
    rdfs:comment "A cognitive bias, the influence of a particular reference point or anchor on peoples decisions. Often more fully referred to as anchoring-and-adjustment, or anchoring-and-adjusting: after an anchor is set, people adjust insufficiently from that anchor point to arrive at a final answer. Decision makers are biased towards an initially presented value."@en ;
    rdfs:label "anchoring bias"@en ;
    rdfs:subClassOf :IndividualBias .

:RankingBias rdf:type owl:Class ;
    terms:source "https://bioportal.bioontology.org/ontologies/AIO/?p=classes&conceptid=https%3A%2F%2Fw3id.org%2Faio%2FRankingBias"@en ;
    rdfs:comment "The idea that top-ranked results are the most relevant and important and will result in more clicks than other results."@en ;
    rdfs:label "ranking bias"@en ;
    rdfs:subClassOf :AnchoringBias .

:AnnotatorReportingBias rdf:type owl:Class ;
    terms:source "https://bioportal.bioontology.org/ontologies/AIO/?p=classes&conceptid=https%3A%2F%2Fw3id.org%2Faio%2FAnnotatorReportingBias"@en ;
    rdfs:comment "When users rely on automation as a heuristic replacement for their own information seeking and processing. A form of individual bias but often discussed as a group bias, or the larger effects on natural language processing models."@en ;
    rdfs:label "annotator reporting bias"@en ;
    rdfs:subClassOf :IndividualBias .

:AutomationComplacencyBias rdf:type owl:Class ;
    terms:source "https://bioportal.bioontology.org/ontologies/AIO/?p=classes&conceptid=https%3A%2F%2Fw3id.org%2Faio%2FAutomationComplacencyBias"@en ;
    rdfs:comment "A mental shortcut whereby people tend to overweight what comes easily or quickly to mind, meaning that what is easier to recalle.g., more availablereceives greater emphasis in judgement and decision-making."@en ;
    rdfs:label "automation complacency bias"@en ;
    rdfs:subClassOf :IndividualBias .

:AvailabilityHeuristicBias rdf:type owl:Class ;
    terms:source "https://bioportal.bioontology.org/ontologies/AIO/?p=classes&conceptid=https%3A%2F%2Fw3id.org%2Faio%2FAvailabilityHeuristicBias"@en ;
    rdfs:comment "A mental shortcut whereby people tend to overweight what comes easily or quickly to mind, meaning that what is easier to recalle.g., more availablereceives greater emphasis in judgement and decision-making."@en ;
    rdfs:label "availability heuristic bias"@en ;
    rdfs:subClassOf :IndividualBias .

:BehaviouralBias rdf:type owl:Class ;
    terms:source "https://bioportal.bioontology.org/ontologies/AIO/?p=classes&conceptid=https%3A%2F%2Fw3id.org%2Faio%2FBehavioralBias"@en ;
    rdfs:comment "Systematic distortions in user behavior across platforms or contexts, or across users represented in different datasets."@en ;
    rdfs:label "behavioural bias"@en ;
    rdfs:subClassOf :IndividualBias .

:ConfirmationBias rdf:type owl:Class ;
    terms:source "https://bioportal.bioontology.org/ontologies/AIO/?p=classes&conceptid=https%3A%2F%2Fw3id.org%2Faio%2FConfirmationBias"@en ;
    rdfs:comment "A cognitive bias where people tend to prefer information that aligns with, or confirms, their existing beliefs. People can exhibit confirmation bias in the search for, interpretation of, and recall of information. In the famous Wason selection task experiments, participants repeatedly showed a preference for confirmation over falsification. They were tasked with identifying an underlying rule that applied to number triples they were shown, and they overwhelmingly tested triples that confirmed rather than falsified their hypothesized rule."@en ;
    rdfs:label "confirmation bias"@en ;
    rdfs:subClassOf :IndividualBias .

:DunningKrugerEffectBias rdf:type owl:Class ;
    terms:source "https://bioportal.bioontology.org/ontologies/AIO/?p=classes&conceptid=https%3A%2F%2Fw3id.org%2Faio%2FDunning-KrugerEffectBias"@en ;
    rdfs:comment "The tendency of people with low ability in a given area or task to overestimate their self-assessed ability. Typically measured by comparing self-assessment with objective performance, often called subjective ability and objective ability, respectively."@en ;
    rdfs:label "Dunning-Kruger effect bias"@en ;
    rdfs:subClassOf :IndividualBias .

:ConsumerBias rdf:type owl:Class ;
    terms:source "https://bioportal.bioontology.org/ontologies/AIO/?p=classes&conceptid=https%3A%2F%2Fw3id.org%2Faio%2FConsumerBias"@en ;
    rdfs:comment "Arises when an algorithm or platform provides users with a new venue within which to express their biases, and may occur from either side, or party, in a digital interaction.."@en ;
    rdfs:label "consumer bias"@en ;
    rdfs:subClassOf :IndividualBias .

:HumanReportingBias rdf:type owl:Class ;
    terms:source "https://bioportal.bioontology.org/ontologies/AIO/?p=classes&conceptid=https%3A%2F%2Fw3id.org%2Faio%2FHumanReportingBias"@en ;
    rdfs:comment "When users rely on automation as a heuristic replacement for their own information seeking and processing."@en ;
    rdfs:label "human reporting bias"@en ;
    rdfs:subClassOf :IndividualBias .

:ImplicitBias rdf:type owl:Class ;
    terms:source "https://bioportal.bioontology.org/ontologies/AIO/?p=classes&conceptid=https%3A%2F%2Fw3id.org%2Faio%2FImplicitBias"@en ;
    rdfs:comment "An unconscious belief, attitude, feeling, association, or stereotype that can affect the way in which humans process information, make decisions, and take actions."@en ;
    rdfs:label "implicit bias"@en ;
    rdfs:subClassOf :IndividualBias .

:InterpretationBias rdf:type owl:Class ;
    terms:source "https://bioportal.bioontology.org/ontologies/AIO/?p=classes&conceptid=https%3A%2F%2Fw3id.org%2Faio%2FInterpretationBias"@en ;
    rdfs:comment "A form of information processing bias that can occur when users interpret algorithmic outputs according to their internalized biases and views."@en ;
    rdfs:label "interpretation bias"@en ;
    rdfs:subClassOf :IndividualBias .

:LossOfSituationalAwarenessBias rdf:type owl:Class ;
    terms:source "https://bioportal.bioontology.org/ontologies/AIO/?p=classes&conceptid=https%3A%2F%2Fw3id.org%2Faio%2FLossOfSituationalAwarenessBias"@en ;
    rdfs:comment "When automation leads to humans being unaware of their situation such that, when control of a system is given back to them in a situation where humans and machines cooperate, they are unprepared to assume their duties. This can be a loss of awareness over what automation is and isnt taking care of."@en ;
    rdfs:label "loss of situational awareness bias"@en ;
    rdfs:subClassOf :IndividualBias .

:ModeConfusionBias rdf:type owl:Class ;
    terms:source "https://bioportal.bioontology.org/ontologies/AIO/?p=classes&conceptid=https%3A%2F%2Fw3id.org%2Faio%2FModeConfusionBias"@en ;
    rdfs:comment "When modal interfaces confuse human operators, who misunderstand which mode the system is using, taking actions which are correct for a different mode but incorrect for their current situation. This is the cause of many deadly accidents, but also a source of confusion in everyday life."@en ;
    rdfs:label "mode confusion bias"@en ;
    rdfs:subClassOf :IndividualBias .

:PresentationBias rdf:type owl:Class ;
    terms:source "https://bioportal.bioontology.org/ontologies/AIO/?p=classes&conceptid=https%3A%2F%2Fw3id.org%2Faio%2FPresentationBias"@en ;
    rdfs:comment "Biases arising from how information is presented on the Web, via a user interface, due to rating or ranking of output, or through users own self-selected, biased interaction."@en ;
    rdfs:label "presentation bias"@en ;
    rdfs:subClassOf :IndividualBias .

:RashomonEffectBias rdf:type owl:Class ;
    terms:source "https://bioportal.bioontology.org/ontologies/AIO/?p=classes&conceptid=https%3A%2F%2Fw3id.org%2Faio%2FRashomonEffectBias"@en ;
    rdfs:comment "Refers to differences in perspective, memory and recall, interpretation, and reporting on the same event from multiple persons or witnesses."@en ;
    rdfs:label "Rashomon effect bias"@en ;
    rdfs:subClassOf :IndividualBias .

:SelectiveAdherenceBias rdf:type owl:Class ;
    terms:source "https://bioportal.bioontology.org/ontologies/AIO/?p=classes&conceptid=https%3A%2F%2Fw3id.org%2Faio%2FSelectiveAdherenceBias"@en ;
    rdfs:comment "Decision-makers inclination to selectively adopt algorithmic advice when it matches their pre-existing beliefs and stereotypes."@en ;
    rdfs:label "selective adherence bias"@en ;
    rdfs:subClassOf :IndividualBias .

:StreetlightEffectBias rdf:type owl:Class ;
    terms:source "https://bioportal.bioontology.org/ontologies/AIO/?p=classes&conceptid=https%3A%2F%2Fw3id.org%2Faio%2FStreetlightEffectBias"@en ;
    rdfs:comment "A bias whereby people tend to search only where it is easiest to look."@en ;
    rdfs:label "streetlight effect bias"@en ;
    rdfs:subClassOf :IndividualBias .

:UserInteractionBias rdf:type owl:Class ;
    terms:source "https://bioportal.bioontology.org/ontologies/AIO/?p=classes&conceptid=https%3A%2F%2Fw3id.org%2Faio%2FUserInteractionBias"@en ;
    rdfs:comment "Arises when a user imposes their own self-selected biases and behavior during interaction with data, output, results, etc."@en ;
    rdfs:label "user interaction bias"@en ;
    rdfs:subClassOf :IndividualBias .

:InstitutionalBias rdf:type owl:Class ;
    terms:source "https://bioportal.bioontology.org/ontologies/AIO/?p=classes&conceptid=https%3A%2F%2Fw3id.org%2Faio%2FInstitutionalBias"@en ;
    rdfs:comment "In contrast to biases exhibited at the level of individual persons, institutional bias refers to a tendency exhibited at the level of entire institutions, where practices or norms result in the favoring or disadvantaging of certain social groups. Common examples include institutional racism and institutional sexism."@en ;
    rdfs:label "institutional bias"@en ;
    rdfs:subClassOf :CognitiveBias .

:SunkCostFallacyBias rdf:type owl:Class ;
    terms:source "https://bioportal.bioontology.org/ontologies/AIO/?p=classes&conceptid=https%3A%2F%2Fw3id.org%2Faio%2FSunkCostFallacyBias"@en ;
    rdfs:comment "A human tendency where people opt to continue with an endeavor or behavior due to previously spent or invested resources, such as money, time, and effort, regardless of whether costs outweigh benefits. For example, in AI, the sunk cost fallacy could lead development teams and organizations to feel that because they have already invested so much time and money into a particular AI application, they must pursue it to market rather than deciding to end the effort, even in the face of significant technical debt and/or ethical debt."@en ;
    rdfs:label "sunk cost fallacy bias"@en ;
    rdfs:subClassOf :GroupBias .

:SystemicBias rdf:type owl:Class ;
    terms:source "https://bioportal.bioontology.org/ontologies/AIO/?p=classes&conceptid=https%3A%2F%2Fw3id.org%2Faio%2FSystemicBias"@en ;
    rdfs:comment "Biases that result from procedures and practices of particular institutions that operate in ways which result in certain social groups being advantaged or favored and others being disadvantaged or devalued."@en ;
    rdfs:label "systemic bias"@en ;
    rdfs:subClassOf :CognitiveBias .

:HistoricalBias rdf:type owl:Class ;
    terms:source "https://bioportal.bioontology.org/ontologies/AIO/?p=classes&conceptid=https%3A%2F%2Fw3id.org%2Faio%2FHistoricalBias"@en ;
    rdfs:comment "Referring to the long-standing biases encoded in society over time. Related to, but distinct from, biases in historical description, or the interpretation, analysis, and explanation of history. A common example of historical bias is the tendency to view the larger world from a Western or European view."@en ;
    rdfs:label "historical bias"@en ;
    rdfs:subClassOf :DataBias .

######################################
# Description of EU fundamental rights
######################################
:EUFundamentalRight rdf:type owl:Class .

:RightToHumanDignity rdf:type :EUFundamentalRight ;
    terms:source "https://data.europa.eu/eli/treaty/char_2012/art_1/oj"@en ;
    rdfs:comment "Human dignity is inviolable. It must be respected and protected."@en ;
    rdfs:label "Human dignity"@en .

:RightToLife rdf:type :EUFundamentalRight ;
    terms:source "http://data.europa.eu/eli/treaty/char_2012/art_2/oj" ;
    rdfs:comment "1. Everyone has the right to life\n2. No one shall be condemned to the death penalty, or executed."@en ;
    rdfs:label "Right to life"@en .

:RightToPersonalIntegrity rdf:type :EUFundamentalRight ;
    terms:source "http://data.europa.eu/eli/treaty/char_2012/art_3/oj"@en ;
    rdfs:comment "1. Everyone has the right to respect for his or her physical and mental integrity.\n2. In fields of medicine and biology, the following must be respected in particular:\n(a) the free and informed consent of the person concerned, according to the procedures laid down by law;\n(b) the prohibition of eugenic practices, in particular those aiming at the selection of persons;\n(c) the prohibition on making the human body and its parts as such a source of financial gain;\n(d) the prohibition of the reproductive clonong of human beings."@en ;
    rdfs:label "Right to the integrity of the person"@en .

:RightProhibitionOfTorture rdf:type :EUFundamentalRight ;
    terms:source "http://data.europa.eu/eli/treaty/char_2012/art_4/oj"@en ;
    rdfs:comment "No one shall be subjected to torture or to inhuman or degrading treatment or punishment."@en ;
    rdfs:label "Prohibition of torture and inhuman or degrading treatment or punishment"@en .

:RightProhibitionOfSlavery rdf:type :EUFundamentalRight ;
    terms:source "http://data.europa.eu/eli/treaty/char_2012/art_5/oj"@en ;
    rdfs:comment "1. No one shall be held in slavery or servitude.\n2. No one shall be required to perform forced or compulsory labour.\n3. Trafficking in human beings is prohibited."@en ;
    rdfs:label "Prohibition of slavery and forced labour"@en .

:RightToLibertyAndSecurity rdf:type :EUFundamentalRight ;
    terms:source "http://data.europa.eu/eli/treaty/char_2012/art_6/oj"@en ;
    rdfs:comment "Everyone has the right to liberty and security of person."@en ;
    rdfs:label "Right to liberty and security"@en .

:RightPrivacy rdf:type :EUFundamentalRight ;
    terms:source "http://data.europa.eu/eli/treaty/char_2012/art_7/oj"@en ;
    rdfs:comment "Everyone has the right to respect for his or her private and family life, home and communications."@en ;
    rdfs:label "Respect for private and family life"@en .

:RightProtectionPersonalData rdf:type :EUFundamentalRight ;
    terms:source "http://data.europa.eu/eli/treaty/char_2012/art_8/oj"@en ;
    rdfs:comment "1. Everyone has the right to the protection of personal data concerning him or her.\n2. Such data must be processed fairly for specified purposes and on the basis of the consent of the person concerned or some other legitimate basis laid down by law. Everyone has the right of access to data which has been collected concerning him or her, and the right to have it rectified.\n3. Compliance with these results shall be subject to control by an independent authority."@en ;
    rdfs:label "Protection of personal data"@en .

:RightMarriageFamily rdf:type :EUFundamentalRight ;
    terms:source "http://data.europa.eu/eli/treaty/char_2012/art_9/oj"@en ;
    rdfs:comment "The right to marry and the right to found a family shall be guaranteed in accordance with the national laws governing the exercise of these rights."@en ;
    rdfs:label "Right to marry and right to found a family"@en .

:RightFreedomOfThoughtConscienceReligion rdf:type :EUFundamentalRight ;
    terms:source "http://data.europa.eu/eli/treaty/char_2012/art_10/oj"@en ;
    rdfs:comment "1. Everyone has the right to freedom of thought, conscience and religion. This right includes freedom to change religion or belief and freedom, either alone or in community with others and in public or in private, to manifest religion or belief, in worship, teaching, practice and observance.\n2. The right to conscientious objection is recognised, in accordance with the national laws governing the exercise of this right."@en ;
    rdfs:label "Freedom of thought, conscience and religion"@en .

:RightFreedomOfExpressionInformation rdf:type :EUFundamentalRight ;
    terms:source "http://data.europa.eu/eli/treaty/char_2012/art_11/oj"@en ;
    rdfs:comment "1. Everyone has the right to freedom of expression. This shall include freedom to hold opinions and to receive and impart information and ideas without interference by public authority and regardless of frontiers.\n2. The freedom and pluralism of the media shall be respected."@en ;
    rdfs:label "Freedom of expression and information"@en .

:RightAssemblyAssociation rdf:type :EUFundamentalRight ;
    terms:source "http://data.europa.eu/eli/treaty/char_2012/art_12/oj"@en ;
    rdfs:comment "1. Everyone has the right to freedom of peaceful assembly and to freedom of association at all levels, in particular in political, trade union and civic matters, which implies the right of everyone to form and to join trade unions for the protection of his or her interests.\n2. Political parties at Union level contribute to expressing the political will of the citizens of the Union."@en ;
    rdfs:label "Freedom of assembly and of association"@en .

:RightFreedomArtsSciences rdf:type :EUFundamentalRight ;
    terms:source "http://data.europa.eu/eli/treaty/char_2012/art_13/oj"@en ;
    rdfs:comment "The arts and scientific research shall be free of constraint. Academic freedom shall be respected."@en ;
    rdfs:label "Freedom of the arts and sciences"@en .

:RightEducation rdf:type :EUFundamentalRight ;
    terms:source "http://data.europa.eu/eli/treaty/char_2012/art_14/oj"@en ;
    rdfs:comment "1. Everyone has the right to education and to have access to vocational and continuing training.\n2. This right includes the possibility to receive free compulsory education.\n3. The freedom to found educational establishments with due respect for democratic principles and the right of parents to ensure the education and teaching of their children in conformity with their religious, philosophical and pedagogical convictions shall be respected, in accordance with the national laws governing the exercise of such freedom and right."@en ;
    rdfs:label "Right to education"@en .

:RightWork rdf:type :EUFundamentalRight ;
    terms:source "http://data.europa.eu/eli/treaty/char_2012/art_15/oj"@en ;
    rdfs:comment "1. Everyone has the right to engage in work and to pursue a freely chosen or accepted occupation.\n2. Every citizen of the Union has the freedom to seek employment, to work, to exercise the right of establishment and to provide services in any Member State.\n3. Nationals of third countries who are authorised to work in the territories of the Member States are entitled to working conditions equivalent to those of citizens of the Union."@en ;
    rdfs:label "Freedom to choose an occupation and right to engage in work"@en .

:RightBusiness rdf:type :EUFundamentalRight ;
    terms:source "http://data.europa.eu/eli/treaty/char_2012/art_16/oj"@en ;
    rdfs:comment "The freedom to conduct a business in accordance with Union law and national laws and practices is recognised."@en ;
    rdfs:label "Freedom to conduct a business"@en .

:RightProperty rdf:type :EUFundamentalRight ;
    terms:source "http://data.europa.eu/eli/treaty/char_2012/art_17/oj"@en ;
    rdfs:comment "1. Everyone has the right to own, use, dispose of and bequeath his or her lawfully acquired possessions. No one may be deprived of his or her possessions, except in the public interest and in the cases and under the conditions provided for by law, subject to fair compensation being paid in good time for their loss. The use of property may be regulated by law in so far as is necessary for the general interest.\n2. Intellectual property shall be protected."@en ;
    rdfs:label "Right to property"@en .

:RightAsylum rdf:type :EUFundamentalRight ;
    terms:source "http://data.europa.eu/eli/treaty/char_2012/art_18/oj"@en ;
    rdfs:comment "The right to asylum shall be guaranteed with due respect for the rules of the Geneva Convention of 28 July 1951 and the Protocol of 31 January 1967 relating to the status of refugees and in accordance with the Treaty on European Union and the Treaty on the Functioning of the European Union (hereinafter referred to as 'the Treaties')."@en ;
    rdfs:label "Right to asylum"@en .

:RightProtection rdf:type :EUFundamentalRight ;
    terms:source "http://data.europa.eu/eli/treaty/char_2012/art_19/oj"@en ;
    rdfs:comment "1. Collective expulsions are prohibited.\n2. No one may be removed, expelled or extradited to a State where there is a serious risk that he or she would be subjected to the death penalty, torture or other inhuman or degrading treatment or punishment."@en ;
    rdfs:label "Protection in the event of removal, expulsion or extradition"@en .

:RightEqualityLaw rdf:type :EUFundamentalRight ;
    terms:source "http://data.europa.eu/eli/treaty/char_2012/art_20/oj"@en ;
    rdfs:comment "Everyone is equal before the law."@en ;
    rdfs:label "Equality before the law"@en .

:RightNonDiscrimination rdf:type :EUFundamentalRight ;
    terms:source "http://data.europa.eu/eli/treaty/char_2012/art_21/oj"@en ;
    rdfs:comment "1. Any discrimination based on any ground such as sex, race, colour, ethnic or social origin, genetic features, language, religion or belief, political or any other opinion, membership of a national minority, property, birth, disability, age or sexual orientation shall be prohibited.\n2. Within the scope of application of the Treaties and without prejudice to any of their specific provisions, any discrimination on grounds of nationality shall be prohibited."@en ;
    rdfs:label "Non-discrimination"@en .

:RightDiversity rdf:type :EUFundamentalRight ;
    terms:source "http://data.europa.eu/eli/treaty/char_2012/art_22/oj"@en ;
    rdfs:comment "The Union shall respect cultural, religious and linguistic diversity."@en ;
    rdfs:label "Cultural, religious and linguistic diversity"@en .

:RightGenderEquality rdf:type :EUFundamentalRight ;
    terms:source "http://data.europa.eu/eli/treaty/char_2012/art_23/oj"@en ;
    rdfs:comment "Equality between women and men must be ensured in all areas, including employment, work and pay.\nThe principle of equality shall not prevent the maintenance or adoption of measures providing for specific advantages in favour of the under-represented sex."@en ;
    rdfs:label "Equality between women and men"@en .

:RightChild rdf:type :EUFundamentalRight ;
    terms:source "http://data.europa.eu/eli/treaty/char_2012/art_24/oj"@en ;
    rdfs:comment "1. Children shall have the right to such protection and care as is necessary for their well-being. They may express their views freely. Such views shall be taken into consideration on matters which conern them in accordance with their age and maturity.\n2. In all actions relating to children, where taken by public authorities or private institutions, the child's best interests must be a primary consideration.\n3. Every child shall have the right to maintain on a regular basis a personal relationship and direct contact with both his or her parents, unless that is contrary to his or her interests."@en ;
    rdfs:label "The rights of the child"@en .

:RightElderly rdf:type :EUFundamentalRight ;
    terms:source "http://data.europa.eu/eli/treaty/char_2012/art_25/oj"@en ;
    rdfs:comment "The Union recognises and respects the rights of the elderly to lead a life of dignity and independence and to participate in social and cultural life."@en ;
    rdfs:label "The rights of the elderly"@en .

:RightPersonWithDisabilities rdf:type :EUFundamentalRight ;
    terms:source "http://data.europa.eu/eli/treaty/char_2012/art_26/oj"@en ;
    rdfs:comment "The Union recognises and respects the right of persons with disabilities to benefit from measures designed to ensure their independence, social and occupational integration and participation in the life of the community."@en ;
    rdfs:label "Integration of persons with disabilities"@en .

:RightWorkerInformationConsultation rdf:type :EUFundamentalRight ;
    terms:source "http://data.europa.eu/eli/treaty/char_2012/art_27/oj"@en ;
    rdfs:comment "Workers or their representatives must, at the appropriate levels, be guaranteed information and consultation in good time in the cases and under the conditions provided for by Union law and national laws and practices."@en ;
    rdfs:label "Workers' right to information and consultation within the undertaking"@en .

:RightCollectiveBargainingAction rdf:type :EUFundamentalRight ;
    terms:source "http://data.europa.eu/eli/treaty/char_2012/art_28/oj"@en ;
    rdfs:comment "Workers and employers, or their respective organisations, have, in accordance with Union law and national laws and practices, the right to negotiate and conclude collective agreements at the appropriate levels and, in cases of conflicts of interest, to take collective action to defend their interests, including strike action."@en ;
    rdfs:label "Right of collective bargaining and action"@en .

:RightPlacementServices rdf:type :EUFundamentalRight ;
    terms:source "http://data.europa.eu/eli/treaty/char_2012/art_29/oj"@en ;
    rdfs:comment "Everyone has the right of access to a free placement service."@en ;
    rdfs:label "Right of access to placement services"@en .

:RightProtectionUnjustifiedDismissal rdf:type :EUFundamentalRight ;
    terms:source "http://data.europa.eu/eli/treaty/char_2012/art_30/oj"@en ;
    rdfs:comment "Every worker has the right to protection against unjustified dismissal, in accordance with Union law and national laws and practices."@en ;
    rdfs:label "Protection in the event of unjustified dismissal"@en .

:RightFairWorkingConditions rdf:type :EUFundamentalRight ;
    terms:source "http://data.europa.eu/eli/treaty/char_2012/art_31/oj"@en ;
    rdfs:comment "1. Every worker has the right to working conditions which respect his or her health, safety and dignity.\n2. Every worker has the right to limitation of maximum working hours, to daily and weekly rest periods and to an annual period of paid leave."@en ;
    rdfs:label "Fair and just working conditions"@en .

:RightProhibitionChildLabour rdf:type :EUFundamentalRight ;
    terms:source "http://data.europa.eu/eli/treaty/char_2012/art_32/oj"@en ;
    rdfs:comment "The employment of children is prohibited. The minimum age of admission to employment may not be lower than the minimum school-leaving age, without prejudice to such rules as may be more favourable to young people and except for limited derogations.\nYoung people admitted to work must have working conditions appropriate to their age and be protected against economic exploitation and any work likely to harm their safety, health or physical, mental, moral or social development or to interfere with their education."@en ;
    rdfs:label "Prohibition of child labour and protection of young people at work"@en .

:RightFamilyProfessionalLife rdf:type :EUFundamentalRight ;
    terms:source "http://data.europa.eu/eli/treaty/char_2012/art_33/oj"@en ;
    rdfs:comment "1. The family shall enjoy legal, economic and social protection.\n2. To reconcile family and professional life, everyone shall have the right to protection from dismissal for a reason connected with maternity and the right to paid maternity leave and to parential leave following the birth or adoption of a child."@en ;
    rdfs:label "Family and professional life"@en .

:RightSocialSecurityAssistance rdf:type :EUFundamentalRight ;
    terms:source "http://data.europa.eu/eli/treaty/char_2012/art_34/oj"@en ;
    rdfs:comment "1. The Union recognises and respects the entitlement to social security benefits and social services providing protection in cases such as maternity, illness, industrial accidents, dependency or old age, and in the case of loss of employment, in accordance with the rules laid down by Union law and national laws and practices.\n2. Everyone residing and moving legally within the European Union is entitled to social security benefits and social advantages in accordance with Union law and national laws and practices.\n3. In order to combat social exclusion and poverty, the Union recognises and respects the right to social and housing assistance so as to ensure a decent existence for all those who lack sufficient resources, in accordance with the rules laid down by Union law and national laws and practices."@en ;
    rdfs:label "Social security and social assistance"@en .

:RightHealthcare rdf:type :EUFundamentalRight ;
    terms:source "http://data.europa.eu/eli/treaty/char_2012/art_35/oj"@en ;
    rdfs:comment "Everyone has the right of access to preventive health care and the right to benefit from medical treatment under the conditions established by national laws and practices. A high level of human health protection shall be ensured in the definition and implementation of all the Union's policies and activities."@en ;
    rdfs:label "Health care"@en .

:RightAccessServicesEconomicInterest rdf:type :EUFundamentalRight ;
    terms:source "http://data.europa.eu/eli/treaty/char_2012/art_36/oj"@en ;
    rdfs:comment "The Union recognises and respects access to services of general economic interest as provided for in national laws and practices, in accordance with the Treaties, in order to promote the social and territorial cohesion of the Union."@en ;
    rdfs:label "Access to services of general economic interest"@en .

:RightEnvironmentalProtection rdf:type :EUFundamentalRight ;
    terms:source "http://data.europa.eu/eli/treaty/char_2012/art_37/oj"@en ;
    rdfs:comment "A high level of envioronmental protection and the improvement of the quality of the environment must be integrated into the policies of the Union and ensured in accordance with the principle of sustainable development."@en ;
    rdfs:label "Environmental protection"@en .

:RightConsumerProtection rdf:type :EUFundamentalRight ;
    terms:source "http://data.europa.eu/eli/treaty/char_2012/art_38/oj" ;
    rdfs:comment "Union policies shall ensure a high level of consumer protection."@en ;
    rdfs:label "Consumer protection"@en .

:RightVoteAndCandidacyEU rdf:type :EUFundamentalRight ;
    terms:source "http://data.europa.eu/eli/treaty/char_2012/art_39/oj"@en ;
    rdfs:comment "1. Every citizen of the Union has the right to vote and to stand as a candidate at elections to the European Parliament in the Member State in which he or she resides, under the same conditions as nationals of that State.\n2. Members of the European Parliament shall be elected by direct universal suffrage in a free and secret ballot."@en ;
    rdfs:label "Right to vote and to stand as a candidate at elections to the European Parliament"@en .

:RightVoteAndCandidacyMunicipal rdf:type :EUFundamentalRight ;
    terms:source "http://data.europa.eu/eli/treaty/char_2012/art_40/oj"@en ;
    rdfs:comment "Every citizen of the Union has the right to vote and to stand as a candidate at municipal elections in the Member State in which he or she resides under the same conditions as nationals of that State."@en ;
    rdfs:label "Right to vote and to stand as a candidate at municipal elections"@en .

:RightGoodAdministration rdf:type :EUFundamentalRight ;
    terms:source "http://data.europa.eu/eli/treaty/char_2012/art_41/oj"@en ;
    rdfs:comment "1. Every person has the right to have his or her affairs handled impartially, fairly and within a reasonable time by the institutions, bodies, offices and agencies of the Union.\n2. This right includes:\n(a) the right of every person to be heard, before any individual measure which would affect him or her adversely is taken;\n(b) the right of every person to have access to his or her file, while respecting the legitimate interests of confidentiality and of professional and business secrecy;\n(c) the obligation of the administration to give reasons for its decisions.\n3. Every person has the right to have the Union make good any damage caused by its institutions or by its servants in the performance of their duties, in accordance with the geeneral principles common to the laws of the Member States.\n4. Every person may write to the institutions of the Union in one of the languages of the Treaties and must have an answer in the same language."@en ;
    rdfs:label "Right to good administration"@en .

:RightAccessDocuments rdf:type :EUFundamentalRight ;
    terms:source "http://data.europa.eu/eli/treaty/char_2012/art_42/oj"@en ;
    rdfs:comment "Any citizen of the Union, and any natural or legal person residing or having its registered office in a Member State, has a right of access to documents of the institutions, bodies, offices and agencies of the Union, whatever their medium."@en ;
    rdfs:label "Right of access to documents"@en .

:RightOmbudsman rdf:type :EUFundamentalRight ;
    terms:source "http://data.europa.eu/eli/treaty/char_2012/art_43/oj"@en ;
    rdfs:comment "Any citizen of the Union and any natural or legal person residing or having its registered office in a Member State has the right to refer to the European Ombudsman cases of maladministration in the activities of the institutions, bodies, offices or agencies of the Union, with the exception of the Court of Justice of the European Union acting in its judicial role."@en ;
    rdfs:label "European Ombudsman"@en .

:RightPetition rdf:type :EUFundamentalRight ;
    terms:source "http://data.europa.eu/eli/treaty/char_2012/art_44/oj"@en ;
    rdfs:comment "Any citizen of the Union and any natural or legal person residing or having its registered office in a Member State has the right to petition the European Parliament."@en ;
    rdfs:label "Right to petition"@en .

:RightFreedomMovementResidence rdf:type :EUFundamentalRight ;
    terms:source "http://data.europa.eu/eli/treaty/char_2012/art_45/oj"@en ;
    rdfs:commnet "1. Every citizen of the Union has the right to move and reside freely within the territory of the Member States.\n2. Freedom of movement and residence may be granted, in accordance with the Treaties, to nationals of third countries legally resident in the territory of a Member State."@en ;
    rdfs:label "Freedom of movement and of residence"@en .

:RightDiplomaticConsularProtection rdf:type :EUFundamentalRight ;
    terms:source "http://data.europa.eu/eli/treaty/char_2012/art_46/oj"@en ;
    rdfs:comment "Every citizen of the Union shall, in the territory of a third country in which the Member State of which he or she is a national is not represented, be entitled to protection by the diplomatic or consular authorities of any Member State, on the same conditions as the nationals of that Member State."@en ;
    rdfs:label "Diplomatic and consular protection"@en .

:RightRemedyFairTrial rdf:type :EUFundamentalRight ;
    terms:source "http://data.europa.eu/eli/treaty/char_2012/art_47/oj"@en ;
    rdfs:comment "Everyone whose rights and freedoms guaranteed by the law of the Union are violated has the right to an effective remedy before a tribunal in compliance with the conditions laid down in this Article.\nEveryone is entitled to a fair and public hearing within a reasonable time by an independent and impartial tribunal previously established by law. Everyone shall have the possibility of being advised, defended and represented.\nLegal aid shall be made available to those who lack sufficient resources in so far as such aid is necessary to ensure effective access to justice."@en ;
    rdfs:label "Right to an effective remedy and to a fair trial"@en .

:RightPresumptionInnocence rdf:type :EUFundamentalRight ;
    terms:source "http://data.europa.eu/eli/treaty/char_2012/art_48/oj"@en ;
    rdfs:comment "1. Everyone who has been charged shall be presumed innocent until proved guilty according to law.\n2. Respect for the rights of the defence of anyone who has been charged shall be guaranteed."@en ;
    rdfs:label "Presumption of innocence and right of defence"@en .

:PrinciplesLegalityProportionality rdf:type :EUFundamentalRight ;
    terms:source "http://data.europa.eu/eli/treaty/char_2012/art_49/oj"@en ;
    rdfs:comment "1. No one shall be held guilty of any criminal offence on account of any act or omission which did not constitute a criminal offence under national law or international law at the time when it was committed. Nor shall a heavier penalty be imposed than the one that was applicable at the time the criminal offence was committed. If, subsequent to the commission of a criminal offence, the law provides for a lighter penalty, that penalty shall be applicable.\n2. This Article shall not prejudice the trial and punishment of any person for any act or omission which, at the time when it was committed, was criminal according to the general principles recognised by the community of nations.\n3. The severity of penalties must not be disproportionate to the criminal offence."@en ;
    rdfs:label "Principles of legality and proportionality of criminal offences and penalties"@en .

:RightNoPunishmentTwice rdf:type :EUFundamentalRight ;
    terms:source "http://data.europa.eu/eli/treaty/char_2012/art_50/oj"@en ;
    rdfs:comment "No one shall be liable to be tried or punished again in criminal proceedings for an offence for which he or she has already been finally acquitted or convicted within the Union in accordance with the law."@en ;
    rdfs:label "Right not to be tried or punished twice in criminal proceedings for the same criminal offence"@en .

:interpretedBias rdf:type owl:ObjectProperty ;
    rdfs:domain :BiasAudit ;
    rdfs:range :Bias ;
    rdfs:comment "Indicates a bias type interpreted from a bias audit"@en ;
    rdfs:label "Interpreted bias"@en .

# 'Potentially violates' to associate bias assertions with potential breaches of EU fundamental rights
:potentiallyViolates rdf:type owl:ObjectProperty ;
    rdfs:domain :SocietalBias ;
    rdfs:range :EUFundamentalRight ;
    rdfs:comment "Connects a societal bias with a potential violation of an EU fundamental right." ;
    rdfs:label "potentially violates" .

# Some potential violations of EU fundamental rights.
# Gender bias
:GenderBias :potentiallyViolates :RightGenderEquality ,
    :RightNonDiscrimination ,
    :RightWork ,
    :RightFairWorkingConditions .

# Relgious bias
:ReligionBias :potentiallyViolates :RightFreedomOfThoughtConscienceReligion ,
    :RightNonDiscrimination ,
    :RightDiversity .

# Racial bias
:RacialBias :potentiallyViolates :RightNonDiscrimination ,
    :RightToHumanDignity ,
    :RightWork ,
    :RightEducation .

# Sexual orientation bias
:SexualOrientationBias :potentiallyViolates :RightNonDiscrimination ,
    :RightPrivacy ,
    :RightMarriageFamily .

# Ethnic bias
:EthnicBias :potentiallyViolates :RightNonDiscrimination ,
    :RightPrivacy ,
    :RightMarriageFamily ,
    :RightWork .

# Political bias
:PoliticalBias :potentiallyViolates :RightFreedomOfExpressionInformation ,
    :RightAssemblyAssociation ,
    :RightNonDiscrimination .

# Philosophical belief bias
:PhilosophicalBeliefBias :potentiallyViolates :RightFreedomOfThoughtConscienceReligion ,
    :RightNonDiscrimination ,
    :RightEducation .

# Trade union membership
:TradeUnionMembershipBias :potentiallyViolates :RightAssemblyAssociation ,
    :RightCollectiveBargainingAction ,
    :RightWork .

# Genetic data bias
:GeneticDataBias :potentiallyViolates :RightProtectionPersonalData ,
    :RightPrivacy ,
    :RightNonDiscrimination ,
    :RightHealthcare .

# Biometric data use
:BiometricDataUseBias :potentiallyViolates :RightProtectionPersonalData ,
    :RightPrivacy ,
    :RightToPersonalIntegrity .

# Health data bias
:HealthDataBias :potentiallyViolates :RightProtectionPersonalData ,
    :RightPrivacy ,
    :RightHealthcare ,
    :RightNonDiscrimination .

# Has purpose
:PurposeDimension rdf:type dqv:Dimension ;
	terms:source "Datasheets for datasets, https://arxiv.org/pdf/1803.09010."@en ;
	rdfs:label "Purpose of dataset"@en ;
	rdfs:comment "Describes for what purpose was the dataset created."@en .

:PurposeMetric rdf:type dqv:Metric ;
	rdfs:comment "A metric to measure the purpose dimension of a dataset"@en ;
	rdfs:label "se metric"@en ;
	dqv:inDimension :PurposeDimension .

# Funded by
:FundingPresenceDimension rdf:type dqv:Dimension ;
	terms:source "Datasheets for datasets, https://arxiv.org/pdf/1803.09010."@en ;
    rdfs:label "Funding presence"@en ;
    rdfs:comment "Indicates whether funding was received for a particular dataset"@en .

:FundingDescriptionDimension rdf:type dqv:Dimension ;
	terms:source "Datasheets for datasets, https://arxiv.org/pdf/1803.09010."@en ;
    rdfs:label "Funding description"@en ;
    rdfs:comment "Describes dataset funding, if present."@en .

:FundingPresenceMetric rdf:type dqv:Metric ;
	rdfs:comment "A metric to measure the funding presence dimension of a dataset"@en ;
	rdfs:label "Funding presence metric"@en ;
	dqv:inDimension :FundingPresenceDimension .

:FundingDescriptionMetric rdf:type dqv:Metric ;
	rdfs:comment "A metric to measure the funding description dimension of a dataset"@en ;
	rdfs:label "Funding description metric"@en ;
	dqv:inDimension :FundingDescriptionDimension .


# Comprised of instances
:InstanceTypesDimension rdf:type dqv:Dimension ;
	terms:source "Datasheets for datasets, https://arxiv.org/pdf/1803.09010."@en ;
	rdfs:label "Instance types"@en ;
	rdfs:comment "Describes the types of instances comprising the dataset"@en .

:InstanceTypesMetric rdf:type dqv:Metric ;
	rdfs:comment "A metric to measure the instance types dimension of a dataset"@en ;
	rdfs:label "Instance types metric"@en ;
	dqv:inDimension :InstanceTypesDimension .


# Number of instances
:InstanceCountDimension rdf:type dqv:Dimension ;
	terms:source "Datasheets for datasets, https://arxiv.org/pdf/1803.09010."@en ;
	rdfs:label "Instance count"@en ;
	rdfs:comment "Counts of instances in the dataset"@en .

:InstanceCountMetric rdf:type dqv:Metric ;
	rdfs:comment "A metric to measure the instance count dimension of a dataset"@en ;
	rdfs:label "Instance count metric"@en ;
	dqv:inDimension :InstanceCountDimension .


# Instances subset or all
:SamplingDimension rdf:type dqv:Dimension ;
	terms:source "Datasheets for datasets, https://arxiv.org/pdf/1803.09010."@en ;
	rdfs:label "Sampling information"@en ;
	rdfs:comment "Indicates if the dataset is complete (i.e., not a sample (of a larger dataset)). In this implementation, 'complete' is interpreted as 'true' (xsd:boolean) and 'sample' is interpreted from 'false' (xsd:boolean)"@en .

:RepresentativenessDimension rdf:type dqv:Dimension ;
	terms:source "Datasheets for datasets, https://arxiv.org/pdf/1803.09010."@en ;
	rdfs:label "Representativeness"@en ;
	rdfs:comment "Describes how representative the sample is of the larger set"@en .

:SamplingMethodDimension rdf:type dqv:Dimension ;
	terms:source "Datasheets for datasets, https://arxiv.org/pdf/1803.09010."@en ;
	rdfs:label "Sampling method"@en ;
	rdfs:comment "Describes the method used for sampling"@en .

:SamplingMetric rdf:type dqv:Metric ;
	rdfs:comment "A metric to measure the sampling dimension of a dataset"@en ;
	rdfs:label "Sampling metric"@en ;
	dqv:inDimension :SamplingDimension .

:RepresentativenessMetric rdf:type dqv:Metric ;
	rdfs:comment "A metric to measure the representativeness dimension of a dataset"@en ;
	rdfs:label "Representativeness metric"@en ;
	dqv:inDimension :RepresentativenessDimension .

:SamplingMethodMetric rdf:type dqv:Metric ;
	rdfs:comment "A metric to measure the sampling method dimension of a dataset"@en ;
	rdfs:label "Sampling method metric"@en ;
	dqv:inDimension :SamplingMethodDimension .


# Each instance consists of
:InstanceCompositionDimension rdf:type dqv:Dimension ;
	terms:source "Datasheets for datasets, https://arxiv.org/pdf/1803.09010."@en ;
	rdfs:label "Instance composition"@en ;
	rdfs:comment "Describes what each instance in the dataset consists of"@en .

:InstanceCompositionMetric rdf:type dqv:Metric ;
	rdfs:comment "A metric to measure the instance composition dimension of a dataset"@en ;
	rdfs:label "Instance composition metric"@en ;
	dqv:inDimension :InstanceCompositionDimension .


# Label or target
:LabelPresenceDimension rdf:type dqv:Dimension ;
	terms:source "Datasheets for datasets, https://arxiv.org/pdf/1803.09010."@en ;
	rdfs:label "Label presence"@en ;
	rdfs:comment "Indicates whether labels or targets are associated with instances."@en .

:LabelDescriptionDimension rdf:type dqv:Dimension ;
	terms:source "Datasheets for datasets, https://arxiv.org/pdf/1803.09010."@en ;
	rdfs:label "Label description"@en ;
	rdfs:comment "Provides a detailed description of the labels or targets associated with instances"@en .

:LabelPresenceMetric rdf:type dqv:Metric ;
	rdfs:comment "A metric to measure the label presence dimension of a dataset"@en ;
	rdfs:label "Label presence metric"@en ;
	dqv:inDimension :LabelPresenceDimension .

:LabelDescriptionMetric rdf:type dqv:Metric ;
	rdfs:comment "A metric to measure the label description dimension of a dataset"@en ;
	rdfs:label "Label description metric"@en ;
	dqv:inDimension :LabelDescriptionDimension .


# Missing information
:MissingInfoPresenceDimension rdf:type dqv:Dimension ;
	terms:source "Datasheets for datasets, https://arxiv.org/pdf/1803.09010."@en ;
	rdfs:label "Presence of missing information"@en ;
	rdfs:comment "Indicates whether any information is missing from individual instances"@en .

:MissingInfoDescriptionDimension rdf:type dqv:Dimension ;
	terms:source "Datasheets for datasets, https://arxiv.org/pdf/1803.09010."@en ;
	rdfs:label "Description of missing information"@en ;
	rdfs:comment "Provides details about what information is missing and why"@en .

:MissingInfoPresenceMetric rdf:type dqv:Metric ;
	rdfs:comment "A metric to measure the missing info presence dimension of a dataset"@en ;
	rdfs:label "Missing info presence metric"@en ;
	dqv:inDimension :MissingInfoPresenceDimension .

:MissingInfoDescriptionMetric rdf:type dqv:Metric ;
	rdfs:comment "A metric to measure the missing info description dimension of a dataset"@en ;
	rdfs:label "Missing info description metric"@en ;
	dqv:inDimension :MissingInfoDescriptionDimension .


# Relationships made explicit
:RelationshipPresenceDimension rdf:type dqv:Dimension ;
	terms:source "Datasheets for datasets, https://arxiv.org/pdf/1803.09010."@en ;
	rdfs:label "Presence of Explicit Relationships"@en ;
	rdfs:comment "Indicates whether relationships between individual instances are made explicit"@en .

:RelationshipDescriptionDimension rdf:type dqv:Dimension ;
	terms:source "Datasheets for datasets, https://arxiv.org/pdf/1803.09010."@en ;
	rdfs:label "Description of Relationships"@en ;
	rdfs:comment "Provides detail about how relationships between instances are made explicit"@en .

:RelationshipPresenceMetric rdf:type dqv:Metric ;
	rdfs:comment "A metric to measure the relationship presence dimension of a dataset"@en ;
	rdfs:label "Relationship presence metric"@en ;
	dqv:inDimension :RelationshipPresenceDimension .

:RelationshipDescriptionMetric rdf:type dqv:Metric ;
	rdfs:comment "A metric to measure the relationship description dimension of a dataset"@en ;
	rdfs:label "Relationship description metric"@en ;
	dqv:inDimension :RelationshipDescriptionDimension .


# Data splits
:DataSplitPresenceDimension rdf:type dqv:Dimension ;
	terms:source "Datasheets for datasets, https://arxiv.org/pdf/1803.09010."@en ;
	rdfs:label "Presence of Recommended Data Splits"@en ;
	rdfs:comment "Indicates whether recommended data splits are provided"@en .

:DataSplitDescriptionDimension rdf:type dqv:Dimension ;
	terms:source "Datasheets for datasets, https://arxiv.org/pdf/1803.09010."@en ;
	rdfs:label "Description of Data Splits"@en ;
	rdfs:comment "Provides details about recommended data splits and their rationale."@en .

:DataSplitPresenceMetric rdf:type dqv:Metric ;
	rdfs:comment "A metric to measure the data split presence dimension of a dataset"@en ;
	rdfs:label "Data split presence metric"@en ;
	dqv:inDimension :DataSplitPresenceDimension .

:DataSplitDescriptionMetric rdf:type dqv:Metric ;
	rdfs:comment "A metric to measure the data split description dimension of a dataset"@en ;
	rdfs:label "Data split description metric"@en ;
	dqv:inDimension :DataSplitDescriptionDimension .


# Errors, noise, redundancies
:DataIssuesPresenceDimension rdf:type dqv:Dimension ;
	terms:source "Datasheets for datasets, https://arxiv.org/pdf/1803.09010."@en ;
	rdfs:label "Presence of data issues"@en ;
	rdfs:comment "Indicates whether there are known errors, sources of noise, or redunancies in the data"@en .

:DataIssuesDescriptionDimension rdf:type dqv:Dimension ;
	terms:source "Datasheets for datasets, https://arxiv.org/pdf/1803.09010."@en ;
	rdfs:label "Description of data issues" ;
	rdfs:comment "Provides details about known errors, sources of noise, and redunancies in the dataset" .

:DataIssuesPresenceMetric rdf:type dqv:Metric ;
	rdfs:comment "A metric to measure the data issues presence dimension of a dataset"@en ;
	rdfs:label "Data issues presence metric"@en ;
	dqv:inDimension :DataIssuesPresenceDimension .

:DataIssuesDescriptionMetric rdf:type dqv:Metric ;
	rdfs:comment "A metric to measure the data issues description dimension of a dataset"@en ;
	rdfs:label "Data issues description metric"@en ;
	dqv:inDimension :DataIssuesDescriptionDimension .


# External resources
:ExternalResourcesDimension rdf:type dqv:Dimension ;
	terms:source "Datasheets for datasets, https://arxiv.org/pdf/1803.09010."@en ;
	rdfs:label "External resources"@en ;
	rdfs:comment "Indicates whether the dataset links to or relies on external resources"@en .

:ExternalResourcesDescriptionDimension rdf:type dqv:Dimension ;
	terms:source "Datasheets for datasets, https://arxiv.org/pdf/1803.09010."@en ;
	rdfs:label "External resources description"@en ;
	rdfs:comment "Descriptions of all external resources and any restrictions associated with them, as well as links or other access points, as appropriate, if the dataset links to or relies on external resources" .

:ResourceGuaranteesDimension rdf:type dqv:Dimension ;
	terms:source "Datasheets for datasets, https://arxiv.org/pdf/1803.09010."@en ;
	rdfs:label "External resource guarantees"@en ;
	rdfs:comment "Describes guarantees about the existence and consistency of external resources over time"@en .

:ArchivalVersionsDimension rdf:type dqv:Dimension ;
	terms:source "Datasheets for datasets, https://arxiv.org/pdf/1803.09010."@en ;
	rdfs:label "Archival versions"@en ;
	rdfs:comment "Describes the availability of offical archival versions of the complete dataset"@en .

:ExternalRestrictionsDimension rdf:type dqv:Dimension ;
	terms:source "Datasheets for datasets, https://arxiv.org/pdf/1803.09010."@en ;
	rdfs:label "External resource restrictions"@en ;
	rdfs:comment "Describes any restrictions associated with the external resources"@en .

:ExternalResourcesMetric rdf:type dqv:Metric ;
	rdfs:comment "A metric to measure the external resources dimension of a dataset"@en ;
	rdfs:label "External resources metric"@en ;
	dqv:inDimension :ExternalResourcesDimension .

:ExternalResourcesDescriptionMetric rdf:type dqv:Metric ;
	rdfs:comment "A metric to measure the external resources description dimension of a dataset"@en ;
	rdfs:label "External resources description metric"@en ;
	dqv:inDimension :ExternalResourcesDescriptionDimension .

:ResourceGuaranteesMetric rdf:type dqv:Metric ;
	rdfs:comment "A metric to measure the resource guarantees dimension of a dataset"@en ;
	rdfs:label "Resource guarantees metric"@en ;
	dqv:inDimension :ResourceGuaranteesDimension .

:ArchivalVersionsMetric rdf:type dqv:Metric ;
	rdfs:comment "A metric to measure the archival versions dimension of a dataset"@en ;
	rdfs:label "Archival versions metric"@en ;
	dqv:inDimension :ArchivalVersionsDimension .

:ExternalRestrictionsMetric rdf:type dqv:Metric ;
	rdfs:comment "A metric to measure the external restrictions dimension of a dataset"@en ;
	rdfs:label "External restrictions metric"@en ;
	dqv:inDimension :ExternalRestrictionsDimension .


# Confidential data
:ConfidentialDataPresenceDimension rdf:type dqv:Dimension ;
	terms:source "Datasheets for datasets, https://arxiv.org/pdf/1803.09010."@en ;
	rdfs:label "Presence of confidential data"@en ;
	rdfs:comment "Indicates whether the dataset contains data that might be considered confidential"@en .

:ConfidentialDataDescriptionDimension rdf:type dqv:Dimension ;
	terms:source "Datasheets for datasets, https://arxiv.org/pdf/1803.09010."@en ;
	rdfs:label "Description of confidential data"@en ;
	rdfs:comment "Provides details about the nature of confidential data in the dataset"@en .

:ConfidentialDataPresenceMetric rdf:type dqv:Metric ;
	rdfs:comment "A metric to measure the confidential data presence dimension of a dataset"@en ;
	rdfs:label "Confidential data presence metric"@en ;
	dqv:inDimension :ConfidentialDataDescriptionDimension .

:ConfidentialDataDescriptionMetric rdf:type dqv:Metric ;
	rdfs:comment "A metric to measure the confidential data description dimension of a dataset"@en ;
	rdfs:label "Confidential data description metric"@en ;
	dqv:inDimension :ConfidentialDataDescriptionDimension .


# Offensive / insulting / threatening / otherwise anxiety causing data
:AnxietyContentPresenceDimension rdf:type dqv:Dimension ;
	terms:source "Datasheets for datasets, https://arxiv.org/pdf/1803.09010."@en ;
	rdfs:label "Presence of potentially offensive or anxiety-causing content"@en ;
	rdfs:comment "Indicates whether the dataset contains data that might be offensive, insulting, threatening, or might cause anxiety if viewed directly"@en .

:AnxietyContentDescriptionDimension rdf:type dqv:Dimension ;
	terms:source "Datasheets for datasets, https://arxiv.org/pdf/1803.09010."@en ;
	rdfs:label "Description of potentially offensive or anxiety-causing content"@en ;
	rdfs:comment "Provides details about the nature of potentially offensive or anxiety-causing content"@en .

:AnxietyContentPresenceMetric rdf:type dqv:Metric ;
	rdfs:comment "A metric to measure the anxiety content presence dimension of a dataset"@en ;
	rdfs:label "Anxiety content presence metric"@en ;
	dqv:inDimension :AnxietyContentPresenceDimension .

:AnxietyContentDescriptionMetric rdf:type dqv:Metric ;
	rdfs:comment "A metric to measure the anxiety content description dimension of a dataset"@en ;
	rdfs:label "Anxiety content description metric"@en ;
	dqv:inDimension :AnxietyContentDescriptionDimension .


# Subpopulations
:SubpopulationPresenceDimension rdf:type dqv:Dimension ;
	terms:source "Datasheets for datasets, https://arxiv.org/pdf/1803.09010."@en ;
	rdfs:label "Presence of identified subpopulations"@en ;
	rdfs:comment "Indicates whether the dataset identifies subpopulations"@en .

:SubpopulationDescriptionDimension rdf:type dqv:Dimension ;
	terms:source "Datasheets for datasets, https://arxiv.org/pdf/1803.09010."@en ;
	rdfs:label "Description of subpopulations"@en ;
	rdfs:comment "Provides details about how subpopulations are identified and their distributions within the dataset"@en .

:SubpopulationPresenceMetric rdf:type dqv:Metric ;
	rdfs:comment "A metric to measure the subpopulation presence dimension of a dataset"@en ;
	rdfs:label "Subpopulation presence metric"@en ;
	dqv:inDimension :SubpopulationPresenceDimension .

:SubpopulationDescriptionMetric rdf:type dqv:Metric ;
	rdfs:comment "A metric to measure the subpopulation description dimension of a dataset"@en ;
	rdfs:label "Subpopulation description metric"@en ;
	dqv:inDimension :SubpopulationDescriptionDimension .


# Identifiable individuals
:IndividualIdentificationPossibilityDimension rdf:type dqv:Dimension ;
	terms:source "Datasheets for datasets, https://arxiv.org/pdf/1803.09010."@en ;
	rdfs:label "Possibility of individual identification"@en ;
	rdfs:comment "Indicates whether it is possible to identify individuals from the dataset, either directly or indirectly"@en .

:IndividualIdentificationDescriptionDimension rdf:type dqv:Dimension ;
	terms:source "Datasheets for datasets, https://arxiv.org/pdf/1803.09010."@en ;
	rdfs:label "Description of individual identification possibilities"@en ;
	rdfs:comment "Provides details about how individuals might be identified from the dataset"@en .

:IndividualIdentificationPossibilityMetric rdf:type dqv:Metric ;
	rdfs:comment "A metric to measure the individual identification possibility dimension of a dataset"@en ;
	rdfs:label "Individual identification possibility metric"@en ;
	dqv:inDimension :IndividualIdentificationPossibilityDimension .

:IndividualIdentificationDescriptionMetric rdf:type dqv:Metric ;
	rdfs:comment "A metric to measure the individual identification description dimension of a dataset"@en ;
	rdfs:label "Individual identification description metric"@en ;
	dqv:inDimension :IndividualIdentificationDescriptionDimension .


# Sensitive data
:SensitiveDataPresenceDimension rdf:type dqv:Dimension ;
	terms:source "Datasheets for datasets, https://arxiv.org/pdf/1803.09010."@en ;
	rdfs:label "Presence of sensitive data"@en ;
	rdfs:comment "Indicates the presence of data which might be considered sensitive"@en .

:SensitiveDataDescriptionDimension rdf:type dqv:Dimension ;
	terms:source "Datasheets for datasets, https://arxiv.org/pdf/1803.09010."@en ;
	rdfs:label "Description of sensitive data"@en ;
	rdfs:comment "Provides details about how data might be considered sensitive."@en .

:SensitiveDataPresenceMetric rdf:type dqv:Metric ;
	rdfs:comment "A metric to measure the sensitive data presence dimension of a dataset"@en ;
	rdfs:label "Sensitive data presence metric"@en ;
	dqv:inDimension :SensitiveDataPresenceDimension .

:SensitiveDataDescriptionMetric rdf:type dqv:Metric ;
	rdfs:comment "A metric to measure the sensitive data description dimension of a dataset"@en ;
	rdfs:label "Sensitive data description metric"@en ;
	dqv:inDimension :SensitiveDataDescriptionDimension .


# Instance data acquisition
:InstanceAcquisitionMeans rdf:type owl:Class ;
	terms:source "Datasheets for datasets, https://arxiv.org/pdf/1803.09010."@en ;
	rdfs:comment "Indicates a category to describe how the data associated with instances was acquired"@en ;
	rdfs:label "Instance acquisition means"@en .

:DirectlyObservable rdf:type :InstanceAcquisitionMeans ;
	terms:source "Datasheets for datasets, https://arxiv.org/pdf/1803.09010."@en ;
	rdfs:comment "Indicates that a dataset instance was acquired from a directly observable source, e.g. raw text or movie ratings"@en ;
	rdfs:label "Directly observable"@en .

:SubjectReported rdf:type :InstanceAcquisitionMeans ;
	terms:source "Datasheets for datasets, https://arxiv.org/pdf/1803.09010."@en ;
	rdfs:comment "Indicates that a dataset instance was acquired via reports from subjects (e.g., survey responses)"@en ;
	rdfs:label "Subject reported"@en .

:IndirectInferenceDerived rdf:type :InstanceAcquisitionMeans ;
	terms:source "Datasheets for datasets, https://arxiv.org/pdf/1803.09010."@en ;
	rdfs:comment "Indicates that a dataset instance was acquired via indirect infererence / derivation from other data (e.g., part-of-speech tags, model-based guesses for age or language)"@en ;
	rdfs:label "Indirectly inferred/derived"@en .

:InstanceAcquisitionDimension rdf:type dqv:Dimension ;
	terms:source "Datasheets for datasets, https://arxiv.org/pdf/1803.09010."@en ;
	rdfs:label "Instance acquisition"@en ;
	rdfs:comment "Indicates how the data was associated with each instance."@en .

:InstanceAcquisitionVerificationPresenceDimension rdf:type dqv:Dimension ;
	terms:source "Datasheets for datasets, https://arxiv.org/pdf/1803.09010."@en ;
	rdfs:comment "Indicates whether it was verified how the data was associated with each instance."@en ;
	rdfs:label "Instance acquisition verification"@en.

:InstanceAcquisitionVerificationDescriptionDimension rdf:type dqv:Dimension ;
	terms:source "Datasheets for datasets, https://arxiv.org/pdf/1803.09010."@en ;
	rdfs:comment "Describes how the data was associated with each instance"@en ;
	rdfs:label "Instance acquisition verification description"@en .

:InstanceAcquisitionMetric rdf:type dqv:Metric ;
	rdfs:comment "A metric to measure the instance acquisition dimension of a dataset"@en ;
	rdfs:label "Instance acquisition metric"@en ;
	dqv:inDimension :InstanceAcquisitionDimension .

:InstanceAcquisitionVerificationPresenceMetric rdf:type dqv:Metric ;
	rdfs:comment "A metric to measure the instance acquisition verification presence dimension of a dataset"@en ;
	rdfs:label "Instance acquisition verification presence metric"@en ;
	dqv:inDimension :InstanceAcquisitionVerificationPresenceDimension .

:InstanceAcquisitionVerificationDescriptionMetric rdf:type dqv:Metric ;
	rdfs:coment "A metric to measure the instance acquisition verification description dimension of a dataset"@en ;
	rdfs:label "Instance acquisition verification description metric"@en ;
	dqv:inDimension :InstanceAcquisitionVerificationDescriptionDimension .


# Data acquisition mechanisms
:DataAcquisitionMechanismDimension rdf:type dqv:Dimension ;
	terms:source "Datasheets for datasets, https://arxiv.org/pdf/1803.09010."@en ;
	rdfs:comment "Indicates what mechanisms or procedures were used to collect the data."@en ;
	rdfs:label "Data acquisition mechanism"@en .

:DataAcquisitionMechanismValidationPresenceDimension rdf:type dqv:Dimension ;
	terms:source "Datasheets for datasets, https://arxiv.org/pdf/1803.09010."@en ;
	rdfs:comment "Indicates whether the data acquisition mechanism was verified"@en ;
	rdfs:label "Data acquisition mechanism validation"@en .

:DataAcquisitionMechanismValidationDescriptionDimension rdf:type dqv:Dimension ;
	terms:source "Datasheets for datasets, https://arxiv.org/pdf/1803.09010."@en ;
	rdfs:comment "Describes how the data acquisition mechanism was verified"@en ;
	rdfs:label "Data acquisition mechanism validation description"@en .

:DataAcquisitionMechanismMetric rdf:type dqv:Metric ;
	rdfs:comment "A metric to measure the data acquisition mechanism dimension of a dataset"@en ;
	rdfs:label "Data acquisition mechanism metric"@en ;
	dqv:inDimension :DataAcquisitionMechanismDimension .

:DataAcquisitionMechanismValidationPresenceMetric rdf:type dqv:Metric ;
	rdfs:comment "A metric to measure the data acquisition mechanism validation presence dimension of a dataset"@en ;
	rdfs:label "Data acquisition mechanism validation presence metric"@en ;
	dqv:inDimension :DataAcquisitionMechanismValidationPresenceDimension .

:DataAcquisitionMechanismValidationDescriptionMetric rdf:type dqv:Metric ;
	rdfs:comment "A metric to measure the data acquisition mechanism validation description dimension of a dataset"@en ;
	rdfs:label "Data acquisition mechanism validation description metric"@en ;
	dqv:inDimension :DataAcquisitionMechanismValidationDescriptionDimension .


# Collection duration
:DatespanDimension rdf:type dqv:Dimension ;
	terms:source "Datasheets for datasets, https://arxiv.org/pdf/1803.09010."@en ;
	rdfs:comment "Indicates the timeframe over which the data was collected"@en ;
	rdfs:label "Datespan dimension"@en .

:DatespanMatchesInstanceDimension rdf:type dqv:Dimension ;
	terms:source "Datasheets for datasets, https://arxiv.org/pdf/1803.09010."@en ;
	rdfs:comment "Indicates whether the data associated with the instances matches the timeframe over which the data was collected"@en ;
	rdfs:label "Datespan matches instance dimension"@en .

:InstanceDateDescriptionDimension rdf:type dqv:Dimension ;
	terms:source "Datasheets for datasets, https://arxiv.org/pdf/1803.09010."@en ;
	rdfs:comment "Describes the timeframe in which the data associated with the instances was created, if the data associated with the instances does not matches the timeframe over which the data was collected"@en ;
	rdfs:label "Instance data creation timeframe"@en .

:DatespanMetric rdf:type dqv:Metric ;
	rdfs:comment "A metric to measure the datespan dimension of a dataset"@en ;
	rdfs:label "Datespan metric"@en ;
	dqv:inDimension :DatespanDimension .

:DatespanMatchesInstanceMetric rdf:type dqv:Metric ;
	rdfs:comment "A metric to measure the datespan matches instance dimension of a dataset"@en ;
	rdfs:label "Datespan matches instance metric"@en ;
	dqv:inDimension :DatespanMatchesInstanceDimension .

:InstanceDateDescriptionMetric rdf:type dqv:Metric ;
	rdfs:comment "A metric to measure the instance date description dimension of a dataset"@en ;
	rdfs:label "Instance date description metric"@en ;
	dqv:inDimension :InstanceDateDescriptionDimension .


# Ethical review
:EthicalReviewPresenceDimension rdf:type dqv:Dimension ;
	terms:source "Datasheets for datasets, https://arxiv.org/pdf/1803.09010."@en ;
	rdfs:comment "Indicates whether an ethical review was conducted"@en ;
	rdfs:label "Ethical review presence"@en .

:EthicalReviewDescriptionDimension rdf:type dqv:Dimension ;
	terms:source "Datasheets for datasets, https://arxiv.org/pdf/1803.09010."@en ;
	rdfs:comment "Describes the ethical review processes, including the outcomes, as well as a link or other access point to any supporting documentation, if an ethical review was conducted on the dataset."@en ;
	rdfs:label "Ethical review description"@en .

:EthicalReviewPresenceMetric rdf:type dqv:Metric ;
	rdfs:comment "A metric to measure the ethical review presence dimension of a dataset"@en ;
	rdfs:label "Ethical review presence metric"@en ;
	dqv:inDimension :EthicalReviewPresenceDimension .

:EthicalReviewDescriptionMetric rdf:type dqv:Metric ;
	rdfs:comment "A metric to measure the ethical review description dimension of a dataset"@en ;
	rdfs:label "Ethical review description metric"@en ;
	dqv:inDimension :EthicalReviewDescriptionDimension .


# Third-party
:ThirdPartyDimension rdf:type dqv:Dimension ;
	terms:source "Datasheets for datasets, https://arxiv.org/pdf/1803.09010."@en ;
	rdfs:comment "Indicates whether data was collected from individuals directly, or obtained via third parties or other sources (e.g. websites)"@en ;
	rdfs:label "Obtained directly or via third-party"@en .

:ThirdPartyMetric rdf:type dqv:Metric ;
	rdfs:comment "A metric to measure the third party dimension of a dataset"@en ;
	rdfs:label "Third party metric"@en ;
	dqv:inDimension :ThirdPartyDimension .


# Provided notification
:ProvidedNotificationPresenceDimension rdf:type dqv:Dimension ;
	terms:source "Datasheets for datasets, https://arxiv.org/pdf/1803.09010."@en ;
	rdfs:comment "Indicates whether individuals in question were notified about the data collection"@en ;
	rdfs:label "Notification provided"@en .

:ProvidedNotificationDescriptionDimension rdf:type dqv:Dimension ;
	terms:source "Datasheets for datasets, https://arxiv.org/pdf/1803.09010."@en ;
	rdfs:comment "Describes how the individuals in question were notified about the data collection, if they were notified"@en ;
	rdfs:label "Notification provided description"@en .

:ProvidedNotificationPresenceMetric rdf:type dqv:Metric ;
	rdfs:comment "A metric to measure the provided notification presence dimension of a dataset"@en ;
	rdfs:label "Provided notification presence metric"@en ;
	dqv:inDimension :ProvidedNotificationPresenceDimension .

:ProvidedNotificationDescriptionMetric rdf:type dqv:Metric ;
	rdfs:comment "A metric to measure the provided notification description dimension of a dataset"@en ;
	rdfs:label "Provided notification description metric"@en ;
	dqv:inDimension :ProvidedNotificationDescriptionDimension .


# Consent obtained
:ConsentObtainedPresenceDimension rdf:type dqv:Dimension ;
	terms:source "Datasheets for datasets, https://arxiv.org/pdf/1803.09010."@en ;
	rdfs:comment "Indicates whether the individuals in question consented to the collection and use of their data"@en ;
	rdfs:label "Consent obtained"@en .

:ConsentObtainedDescriptionDimension rdf:type dqv:Dimension ;
	terms:source "Datasheets for datasets, https://arxiv.org/pdf/1803.09010."@en ;
	rdfs:comment "If consent was obtained, describes how consent was requested and provided, providing a link or other access point to, or otherwise reproducing, the exact language to which the individuals consented."@en ;
	rdfs:label "Consent obtained description"@en .

:ConsentObtainedPresenceMetric rdf:type dqv:Metric ;
	rdfs:comment "A metric to measure the consent obtained presence dimension of a dataset"@en ;
	rdfs:label "Consent obtained presence metric"@en ;
	dqv:inDimension :ConsentObtainedPresenceDimension .

:ConsentObtainedDescriptionMetric rdf:type dqv:Metric ;
	rdfs:comment "A metric to measure the consent obtained description dimension of a dataset"@en ;
	rdfs:label "Consent obtained description metric"@en ;
	dqv:inDimension :ConsentObtainedDescriptionDimension .


# Consent revokation mechanism
:ConsentRevokationPresenceDimension rdf:type dqv:Dimension ;
	terms:source "Datasheets for datasets, https://arxiv.org/pdf/1803.09010."@en ;
	rdfs:comment "Indicates whether a mechanism to revoke consent in the future or for certain uses was provided to users, if consent was obtained."@en ;
	rdfs:label "Consent revokation"@en .

:ConsentRevokationDescriptionDimension rdf:type dqv:Dimension ;
	terms:source "Datasheets for datasets, https://arxiv.org/pdf/1803.09010."@en ;
	rdfs:comment "Describes the consent revokation mechanism provided to individuals if present, as well as a link or other access point to the mechanism (if appropriate)"@en ;
	rdfs:label "Consent revokation description"@en .

:ConsentRevokationPresenceMetric rdf:type dqv:Metric ;
	rdfs:comment "A metric to measure the consent revokation presence dimension of a dataset"@en ;
	rdfs:label "Consent revokation presence dimension"@en ;
	dqv:inDimension :ConsentRevokationPresenceDimension .

:ConsentRevokationDescriptionMetric rdf:type dqv:Metric ;
	rdfs:comment "A metric to measure the consent revokation description dimension of a dataset"@en ;
	rdfs:label "Consent revokation description metric"@en ;
	dqv:inDimension :ConsentRevokationDescriptionDimension .


# Impact analysis
:ImpactAnalysisPresenceDimension rdf:type dqv:Dimension ;
	terms:source "Datasheets for datasets, https://arxiv.org/pdf/1803.09010."@en ;
	rdfs:comment "Indicates whether an analysis of the potential impact of the dataset and its use on data subject (e.g., a data protection impact analysis) has been conducted"@en ;
	rdfs:label "Impact analysis"@en .

:ImpactAnalysisDescriptionDimension rdf:type dqv:Dimension ;
	terms:source "Datasheets for datasets, https://arxiv.org/pdf/1803.09010."@en ;
	rdfs:comment "Describes the impact analysis, if present, including the outcomes, as well as a link or other access point to any supporting documentation"@en ;
	rdfs:label "Impact analysis description"@en .

:ImpactAnalysisPresenceMetric rdf:type dqv:Metric ;
	rdfs:comment "A metric to measure the impact analysis presence dimension of a dataset"@en ;
	rdfs:label "Impact analysis presence metric"@en ;
	dqv:inDimension :ImpactAnalysisPresenceDimension .

:ImpactAnalysisDescriptionMetric rdf:type dqv:Metric ;
	rdfs:comment "A metric to measure the impact analysis description dimension of a dataset"@en ;
	rdfs:label "Impact analysis description metric"@en ;
	dqv:inDimension :ImpactAnalysisDescriptionDimension .


# Preprocessing data
:PreprocessingDataPresenceDimension rdf:type dqv:Dimension ;
	terms:source "Datasheets for datasets, https://arxiv.org/pdf/1803.09010."@en ;
	rdfs:comment "Indicates whether any preprocessing / cleaning / labelling of the data was done (e.g., discretization or bucketing, tokenization, part-of-speech tagging, SIFT feature extraction, removal of instances, processing of missing values)"@en ;
	rdfs:label "Preprocessing / cleaning / labelling"@en .

:PreprocessingDataDescriptionDimension rdf:type dqv:Dimension ;
	terms:source "Datasheets for datasets, https://arxiv.org/pdf/1803.09010."@en ;
	rdfs:comment "Describes the preprocessing / cleaning / labelling which was carried out on the dataset."@en ;
	rdfs:label "Describes how data was preprocessed / cleaned / labelled, if this was done"@en .

:PreprocessingDataPresenceMetric rdf:type dqv:Metric ;
	rdfs:comment "A metric to measure the preprocessing data presence dimension of a dataset"@en ;
	rdfs:label "Preprocessing data presence metric"@en ;
	dqv:inDimension :PreprocessingDataPresenceDimension .

:PreprocessingDataDescriptionMetric rdf:type dqv:Metric ;
	rdfs:comment "A metric to measure the preprocessing data description dimension of a dataset"@en ;
	rdfs:label "Preprocessing data description metric"@en ;
	dqv:inDimension :PreprocessingDataDescriptionDimension .


######################################################
# Raw data saved and software used only required if 
# Preprocessing / cleaning / labelling was carried out
######################################################
# Raw data saved
:RawDataSavedPresenceDimension rdf:type dqv:Dimension ;
	terms:source "Datasheets for datasets, https://arxiv.org/pdf/1803.09010."@en ;
	rdfs:comment "Indicates whether raw data was saved in addition to the preprocessed/cleaned/labelled data (e.g., to support unanticipated future uses)"@en ;
	rdfs:label "Raw data saved"@en .

:RawDataSavedAccessPointDimension rdf:type dqv:Dimension ;
	terms:source "Datasheets for datasets, https://arxiv.org/pdf/1803.09010."@en ;
	rdfs:comment "Provides a link or other access point to the 'raw' data, if raw data was saved"@en ;
	rdfs:label "Raw data link or other access point"@en .

:RawDataSavedPresenceMetric rdf:type dqv:Metric ;
	rdfs:comment "A metric to measure the raw data saved presence dimension of a dataset"@en ;
	rdfs:label "Raw data saved presence metric"@en ;
	dqv:inDimension :RawDataSavedPresenceDimension .

:RawDataSavedAccessPointMetric rdf:type dqv:Metric ;
	rdfs:comment "A metric to measure the raw data saved access point dimension of a dataset"@en ;
	rdfs:label "Raw data saved access point metric"@en ;
	dqv:inDimension :RawDataSavedAccessPointDimension .


# Software available
:SoftwareAvailablePresenceDimension rdf:type dqv:Dimension ;
	terms:source "Datasheets for datasets, https://arxiv.org/pdf/1803.09010."@en ;
	rdfs:comment "Indicates whether the software that was used to preprocess / clean / label the data is available."@en ;
	rdfs:label "Preprocessing software availability"@en .

:SoftwareAvailableAccessPointDimension rdf:type dqv:Dimension ;
	terms:source "Datasheets for datasets, https://arxiv.org/pdf/1803.09010."@en ;
	rdfs:comment "Provides a link or other access point to the software used."@en ;
	rdfs:label "Preprocessing software access point"@en .

:SoftwareAvailablePresenceMetric rdf:type dqv:Metric ;
	rdfs:comment "A metric to measure the software available presence dimension of a dataset"@en ;
	rdfs:label "Software available presence metric"@en ;
	dqv:inDimension :SoftwareAvailablePresenceDimension .

:SoftwareAvailableAccessPointMetric rdf:type dqv:Metric ;
	rdfs:comment "A metric to measure the software available access point dimension of a dataset"@en ;
	rdfs:label "Software available access point metric"@en ;
	dqv:inDimension :SoftwareAvailableAccessPointDimension .


# Tasks used for
:TasksUsedForPresenceDimension rdf:type dqv:Dimension ;
	terms:source "Datasheets for datasets, https://arxiv.org/pdf/1803.09010."@en ;
	rdfs:comment "Indicates whether the dataset has been used for any tasks already"@en ;
	rdfs:label "Dataset used for previous tasks"@en .

:TasksUsedForDescriptionDimension rdf:type dqv:Dimension ;
	terms:source "Datasheets for datasets, https://arxiv.org/pdf/1803.09010."@en ;
	rdfs:comment "Describes the tasks which the dataset has already been used for, if applicable"@en ;
	rdfs:label "Description of previous tasks"@en .

:TasksUsedForPresenceMetric rdf:type dqv:Metric ;
	rdfs:comment "A metric to measure the tasks used for presence dimension of a dataset"@en ;
	rdfs:label "Tasks used for presence metric"@en ;
	dqv:inDimension :TasksUsedForPresenceDimension .

:TasksUsedForDescriptionMetric rdf:type dqv:Metric ;
	rdfs:comment "A metric to measure the tasks used for description dimension of a dataset"@en ;
	rdfs:label "Tasks used for description metric"@en ;
	dqv:inDimension :TasksUsedForDescriptionDimension .


# Links to papers or systems
:RepositoryLinksPresenceDimension rdf:type dqv:Dimension ;
	terms:source "Datasheets for datasets, https://arxiv.org/pdf/1803.09010."@en ;
	rdfs:comment "Indicates whether there is a repository that links to any or all papers or systems that use the dataset"@en ;
	rdfs:label "Links repository"@en .

:RepositoryLinksAccessPointDimension rdf:type dqv:Dimension ;
	terms:source "Datasheets for datasets, https://arxiv.org/pdf/1803.09010."@en ;
	rdfs:comment "Provides a link or other access point to the repository linking any or all papers or systems that use the dataset"@en ;
	rdfs:label "Links repository access point"@en .

:RepositoryLinksPresenceMetric rdf:type dqv:Metric ;
	rdfs:comment "A metric to measure the repository links presence dimension of a dataset"@en ;
	rdfs:label "Repository links presence metric"@en ;
	dqv:inDimension :RepositoryLinksPresenceDimension .

:RepositoryLinksAccessPointMetric rdf:type dqv:Metric ;
	rdfs:comment "A metric to measure the repository links access point dimension of a dataset"@en ;
	rdfs:label "Repository links access point metric"@en ;
	dqv:inDimension :RepositoryLinksAccessPointDimension .


# Other possible tasks
:OtherPossibleTasksPresenceDimension rdf:type dqv:Dimension ;
	terms:source "Datasheets for datasets, https://arxiv.org/pdf/1803.09010."@en ;
	rdfs:comment "Indicates whether there are (other) tasks which the dataset could be used for"@en ;
	rdfs:label "Other possible tasks"@en .

:OtherPossibleTasksDescriptionDimension rdf:type dqv:Dimension ;
	terms:source "Datasheets for datasets, https://arxiv.org/pdf/1803.09010."@en ;
	rdfs:comment "Describes (other) possible tasks, if there are (other) tasks which the dataset could be used for"@en ;
	rdfs:label "Other possible tasks description"@en .

:OtherPossibleTasksPresenceMetric rdf:type dqv:Metric ;
	rdfs:comment "A metric to measure the other possible tasks presence dimension of a dataset"@en ;
	rdfs:label "Other possible tasks presence metric"@en ;
	dqv:inDimension :OtherPossibleTasksPresenceDimension .

:OtherPossibleTasksDescriptionMetric rdf:type dqv:Metric ;
	rdfs:comment "A metric to measure the other possible tasks description dimension of a dataset"@en ;
	rdfs:label "Other possible tasks description metric"@en ;
	dqv:inDimension :OtherPossibleTasksDescriptionDimension .


# Data composition, collection / processing impact
:CompositionCollectionProcessingFutureImpactPresenceDimension rdf:type dqv:Dimension ;
	terms:source "Datasheets for datasets, https://arxiv.org/pdf/1803.09010."@en ;
	rdfs:comment "Indicates whether there is anything about the composition of the dataset or the way it was collected and preprocessed/cleaned/labelled that might impact future uses"@en ;
	rdfs:label "Composition / collection / processing future impact"@en .

:CompositionCollectionProcessingFutureImpactDescriptionDimension rdf:type dqv:Dimension ;
	terms:source "Datasheets for datasets, https://arxiv.org/pdf/1803.09010."@en ;
	rdfs:comment "Describes anything about the composition of the dataset or the way it was collected and preprocessing/cleaned/labelled that migth impact future uses, if applicable"@en ;
	rdfs:label "Description of composition / collectiong / processing future impact"@en .

:CompositionCollectionProcessingFutureImpactPresenceMetric rdf:type dqv:Metric ;
	rdfs:comment "A metric to measure the composition collection processing future impact presence dimension of a dataset"@en ;
	rdfs:label "Composition collection processing future impact presence metric"@en ;
	dqv:inDimension :CompositionCollectionProcessingFutureImpactPresenceDimension .

:CompositionCollectionProcessingFutureImpactDescriptionMetric rdf:type dqv:Metric ;
	rdfs:comment "A metric to measure the composition collection processing future impact description dimension of a dataset"@en ;
	rdfs:label "Composition collection processing future impact description metric"@en ;
	dqv:inDimension :CompositionCollectionProcessingFutureImpactDescriptionDimension .


# Not other possible tasks
:NotToBeUsedForTaskPresenceDimension rdf:type dqv:Dimension ;
	terms:source "Datasheets for datasets, https://arxiv.org/pdf/1803.09010."@en ;
	rdfs:comment "Indicates whether there are tasks for which the dataset should not be used"@en ;
	rdfs:label "Tasks not to be used for"@en .

:NotToBeUsedForTaskDescriptionDimension rdf:type dqv:Dimension ;
	terms:source "Datasheets for datasets, https://arxiv.org/pdf/1803.09010."@en ;
	rdfs:comment "Describes the tasks for which the dataset should not be used, if applicable"@en ;
	rdfs:label "Tasks not to be used for description"@en .

:NotToBeUsedForTaskPresenceMetric rdf:type dqv:Metric ;
	rdfs:comment "A metric to measure the not to be used for task presence dimension of a dataset"@en ;
	rdfs:label "Not to be used for task presence metric"@en ;
	dqv:inDimension :NotToBeUsedForTaskPresenceDimension .

:NotToBeUsedForTaskDescriptionMetric rdf:type dqv:Metric ;
	rdfs:comment "A metric to measure the not to be used for task description dimension of a dataset"@en ;
	rdfs:label "Not to be used for task description metric"@en ;
	dqv:inDimension :NotToBeUsedForTaskDescriptionDimension .


# Third party distribution
:ThirdPartyDistributionPresenceDimension rdf:type dqv:Dimension ;
	terms:source "Datasheets for datasets, https://arxiv.org/pdf/1803.09010."@en ;
	rdfs:comment "Indicates whether the dataset will be distributed to third parties outside of the entity (e.g., company, institution, organisation) on behalf of which the dataset was created"@en ;
	rdfs:label "Third party distribution"@en .

:ThirdPartyDistributionDescriptionDimension rdf:type dqv:Dimension ;
	terms:source "Datasheets for datasets, https://arxiv.org/pdf/1803.09010."@en ;
	rdfs:comment "Describes how the dataset will be distributed to third parties outside of the entity (e.g., company, institution, organisation) on behalf of which the dataset was created, if applicable"@en ;
	rdfs:label "Third party distribution description"@en .

:ThirdPartyDistributionPresenceMetric rdf:type dqv:Metric ;
	rdfs:comment "A metric to measure the third party distribution presence dimension of a dataset"@en ;
	rdfs:label "Third party distribution presence metric"@en ;
	dqv:inDimension :ThirdPartyDistributionPresenceDimension .

:ThirdPartyDistributionDescriptionMetric rdf:type dqv:Metric ;
	rdfs:comment "A metric to measure the third party distribution description dimension of a dataset"@en ;
	rdfs:label "Third party distribution description metric"@en ;
	dqv:inDimension :ThirdPartyDistributionDescriptionDimension .


# Distribution means
:DistributionMeansDimension rdf:type dqv:Dimension ;
	terms:source "Datasheets for datasets, https://arxiv.org/pdf/1803.09010."@en ;
	rdfs:comment "Describes how the dataset will be distributed (e.g., tarball on website, API, GitHub)"@en ;
	rdfs:label "Distribution means"@en .

:hasDOIDimension rdf:type dqv:Dimension ;
	terms:source "Datasheets for datasets, https://arxiv.org/pdf/1803.09010."@en ;
	rdfs:comment "Indicates whether the datasheet has a digital object identifier (DOI)"@en ;
	rdfs:label "Has DOI"@en .

:DOIDimension rdf:type dqv:Dimension ;
	terms:source "Datasheets for datasets, https://arxiv.org/pdf/1803.09010."@en ;
	rdfs:comment "Specifies the DOI for the dataset, if applicable"@en ;
	rdfs:label "Dataset DOI"@en .

:DistributionMeansMetric rdf:type dqv:Metric ;
	rdfs:comment "A metric to measure the distribution means dimension of a dataset"@en ;
	rdfs:label "Distribution means metric"@en ;
	dqv:inDimension :DistributionMeansDimension .

:hasDOIMetric rdf:type dqv:Metric ;
	rdfs:comment "A metric to measure the has DOI dimension of a dataset"@en ;
	rdfs:label "has DOI metric"@en ;
	dqv:inDimension :hasDOIDimension .

:DOIMetric rdf:type dqv:Metric ;
	rdfs:comment "A metric to measure the DOI dimension of a dataset"@en ;
	rdfs:label "DOI metric"@en ;
	dqv:inDimension :DOIDimension .


# Distribution date
:DistributionDateDimension rdf:type dqv:Dimension ;
	terms:source "Datasheets for datasets, https://arxiv.org/pdf/1803.09010."@en ;
	rdfs:comment "Indicates the date that the dataset will be distributed"@en ;
	rdfs:label "Distribution date"@en .

:DistributionDateMetric rdf:type dqv:Metric ;
	rdfs:comment "A metric to measure the distribution date dimension of a dataset"@en ;
	rdfs:label "Distribution date metric"@en ;
	dqv:inDimension :DistributionDateDimension .


# License
:LicensePresenceDimension rdf:type dqv:Dimension ;
	terms:source "Datasheets for datasets, https://arxiv.org/pdf/1803.09010."@en ;
	rdfs:comment "Indicates whether the dataset will be distributed under a copyright or other intellectual property (IP) license, and/or under applicable terms of use (ToU)"@en ;
	rdfs:label "License"@en .

:LicenseDescriptionDimension rdf:type dqv:Dimension ;
	terms:source "Datasheets for datasets, https://arxiv.org/pdf/1803.09010."@en ;
	rdfs:comment "Description of the license and/or ToU, including a link or other access point to, or otherwise reproducing, any relevant licensing terms or ToU, as well as any fees associated with these restrictions"@en ;
	rdfs:label "Description of licesning and/or ToU, including a link or other access point, if applicable"@en .

:LicensePresenceMetric rdf:type dqv:Metric ;
	rdfs:comment "A metric to measure the license presence dimension of a dataset"@en ;
	rdfs:label "License presence metric"@en ;
	dqv:inDimension :LicensePresenceDimension .

:LicenseDescriptionMetric rdf:type dqv:Metric ;
	rdfs:comment "A metric to measure the license description dimension of a dataset"@en ;
	rdfs:label "License description metric"@en ;
	dqv:inDimension :LicenseDescriptionDimension .


# Restrictions on instance data
:InstanceDataRestrictionPresenceDimension rdf:type dqv:Dimension ;
	terms:source "Datasheets for datasets, https://arxiv.org/pdf/1803.09010."@en ;
	rdfs:comment "Indicates whether any third parties imposed IP-based or other restrictions on the data associated with the instances"@en ;
	rdfs:label "Third party restrictions on instance data"@en .

:InstanceDataRestrictionDescriptionDimension rdf:type dqv:Dimension ;
	terms:source "Datasheets for datasets, https://arxiv.org/pdf/1803.09010."@en ;
	rdfs:comment "Describes how third parties impose IP-based or other restrictions on the data associated with the instances, if applicable"@en ;
	rdfs:label "Description of third party restrictions on instance data"@en .

:InstanceDataRestrictionPresenceMetric rdf:type dqv:Metric ;
	rdfs:comment "A metric to measure the instance data restriction presence dimension of a dataset"@en ;
	rdfs:label "Instance data restriction presence metric"@en ;
	dqv:inDimension :InstanceDataRestrictionPresenceDimension .

:InstanceDataRestrictionDescriptionMetric rdf:type dqv:Metric ;
	rdfs:comment "A metric to measure the instance data restriction description dimension of a dataset"@en ;
	rdfs:label "Instance data restriction description metric"@en ;
	dqv:inDimension :InstanceDataRestrictionDescriptionDimension .


# Export controls / regulatory restrictions
:ExportControlRegulatoryRestrictionPresenceDimension rdf:type dqv:Dimension ;
	terms:source "Datasheets for datasets, https://arxiv.org/pdf/1803.09010."@en ;
	rdfs:comment "Indicates whether any export controls or other regulatory restrictions apply to the dataset or to individual instances"@en ;
	rdfs:label "Export controls / regulatory restrictions"@en .

:ExportControlRegulatoryRestrictionDescriptionDimension rdf:type dqv:Dimension ;
	terms:source "Datasheets for datasets, https://arxiv.org/pdf/1803.09010."@en ;
	rdfs:comment "Describes these restrictions, providing a link or other access point to, or otherwise reproducing, any supporting documentation"@en ;
	rdfs:label "Description of export controls / regulatory restrictions, if applicable"@en .

:ExportControlRegulatoryRestrictionPresenceMetric rdf:type dqv:Metric ;
	rdfs:comment "A metric to measure the export control regulatory restriction presence dimension of a dataset"@en ;
	rdfs:label "Export control regulatory restriction presence metric"@en ;
	dqv:inDimension :ExportControlRegulatoryRestrictionPresenceDimension .

:ExportControlRegulatoryRestrictionDescriptionMetric rdf:type dqv:Metric ;
	rdfs:comment "A metric to measure the export control regulatory restriction description dimension of a dataset"@en ;
	rdfs:label "Export control regulatory restriction description metric"@en ;
	dqv:inDimension :ExportControlRegulatoryRestrictionDescriptionDimension .


####################################################
# Consider maintainer and manager contact as
# Subproperties of the dcat:contactPoint property.
####################################################
# Dataset maintainer
:maintainer rdf:type owl:ObjectProperty ;
	terms:source "Datasheets for datasets, https://arxiv.org/pdf/1803.09010."@en ;
	rdfs:comment "Indicates who will be supporting / hosting / maintaining the dataset"@en ;
	rdfs:label "Dataset supporter / host / maintainer"@en ;
	rdfs:subPropertyOf dcat:contactPoint .


# Manager contact means
:managerContact rdf:type owl:ObjectProperty ;
	terms:source "Datasheets for datasets, https://arxiv.org/pdf/1803.09010."@en ;
	rdfs:comment "Indicates how the owner / curator / manager of the dataset can be contacted (e.g., email address)"@en ;
	rdfs:label "Manager contact"@en ;
	rdfs:subPropertyOf dcat:contactPoint .


# Erratum
:ErratumPresenceDimension rdf:type dqv:Dimension ;
	terms:source "Datasheets for datasets, https://arxiv.org/pdf/1803.09010."@en ;
	rdfs:comment "Indicates whether the dataset has an erratum"@en ;
	rdfs:label "has erratum"@en .

:ErratumAccessPointDimension rdf:type dqv:Dimension ;
	terms:source "Datasheets for datasets, https://arxiv.org/pdf/1803.09010."@en ;
	rdfs:comment "Provides a link or other access point to the erratum, if applicable"@en ;
	rdfs:label "Erratum access point"@en .

:ErratumPresenceMetric rdf:type dqv:Metric ;
	rdfs:comment "A metric to measure the erratum presence dimension of a dataset"@en ;
	rdfs:label "Erratum presence metric"@en ;
	dqv:inDimension :ErratumPresenceDimension .

:ErratumAccessPointMetric rdf:type dqv:Metric ;
	rdfs:comment "A metric to measure the erratum access point dimension of a dataset"@en ;
	rdfs:label "Erratum access point metric"@en ;
	dqv:inDimension :ErratumAccessPointDimension .


# Update details
:UpdatePresenceDimension rdf:type dqv:Dimension ;
	terms:source "Datasheets for datasets, https://arxiv.org/pdf/1803.09010."@en ;
	rdfs:comment "Indicates whether the dataset will be updated (e.g., to correct labelling errors, add new instances, delete instances)"@en ;
	rdfs:label "Dataset updates"@en .

:UpdateFrequencyDimension rdf:type dqv:Dimension ;
	terms:source "Datasheets for datasets, https://arxiv.org/pdf/1803.09010."@en ;
	rdfs:comment "Describes how often updates will be communicated to dataset consumers, if applicable"@en ;
	rdfs:label "Dataset updates frequency"@en .

:UpdaterDimension rdf:type dqv:Dimension ;
	terms:source "Datasheets for datasets, https://arxiv.org/pdf/1803.09010."@en ;
	rdfs:comment "Indicates who will be updating the dataset"@en ;
	rdfs:label "Dataset updater"@en .

:UpdateCommunicationDimension rdf:type dqv:Dimension ;
	terms:source "Datasheets for datasets, https://arxiv.org/pdf/1803.09010."@en ;
	rdfs:comment "Describes how updates will be communicated to dataset consumers, if applicable"@en ;
	rdfs:label "Dataset communication means"@en .

:UpdatePresenceMetric rdf:type dqv:Metric ;
	rdfs:comment "A metric to measure the update presence dimension of a dataset"@en ;
	rdfs:label "Update presence metric"@en ;
	dqv:inDimension :UpdatePresenceDimension .

:UpdateFrequencyMetric rdf:type dqv:Metric ;
	rdfs:comment "A metric to measure the update frequency dimension of a dataset"@en ;
	rdfs:label "Update frequency metric"@en ;
	dqv:inDimension :UpdateFrequencyDimension .

:UpdaterMetric rdf:type dqv:Metric ;
	rdfs:comment "A metric to measure the updater dimension of a dataset"@en ;
	rdfs:label "Updater metric"@en ;
	dqv:inDimension :UpdaterDimension .

:UpdateCommunicationMetric rdf:type dqv:Metric ;
	rdfs:comment "A metric to measure the update communication dimension of a dataset"@en ;
	rdfs:label "Update communication metric"@en ;
	dqv:inDimension :UpdateCommunicationDimension .


# Data retention limits
:DataRetentionPresenceDimension rdf:type dqv:Dimension ;
    terms:source "Datasheets for datasets, https://arxiv.org/pdf/1803.09010."@en ;
    rdfs:comment "If the dataset relates to people, indicates whether there are applicable limits on the retention of the data associated with the instances (e.g., were the individuals in question told that their data would be retained for a fixed period of time and then deleted)"@en ;
	rdfs:label "Data retention"@en .

:DataRetentionDescriptionDimension rdf:type dqv:Dimension ;
    terms:source "Datasheets for datasets, https://arxiv.org/pdf/1803.09010."@en ;
    rdfs:comment "Describes data retention limits and how they will be enforced, if applicable"@en ;
	rdfs:label "Data retention description"@en .

:DataRetentionPresenceMetric rdf:type dqv:Metric ;
	rdfs:comment "A metric to measure the data retention presence dimension of a dataset"@en ;
	rdfs:label "Data retention presence metric"@en ;
	dqv:inDimension :DataRetentionPresenceDimension .

:DataRetentionDescriptionMetric rdf:type dqv:Metric ;
	rdfs:comment "A metric to measure the data retention description dimension of a dataset"@en ;
	rdfs:label "Data retention description metric"@en ;
	dqv:inDimension :DataRetentionDescriptionDimension .


# Legacy support
:LegacySupportPresenceDimension rdf:type dqv:Dimension ;
	terms:source "Datasheets for datasets, https://arxiv.org/pdf/1803.09010."@en ;
	rdfs:comment "Indicates whether older versions of the dataset continue to be supported / hosted / maintained"@en ;
	rdfs:label "Legacy support"@en .

# N.B. The following must be filled whether legacy support is enabled or not
:LegacySupportDescriptionDimension rdf:type dqv:Dimension ;
	terms:source "Datasheets for datasets, https://arxiv.org/pdf/1803.09010."@en ;
	rdfs:comment "Description of how legacy versions will or will not be supported / hosted / maintained."@en ;
	rdfs:label "Legacy support description"@en .

:LegacySupportPresenceMetric rdf:type dqv:Metric ;
	rdfs:comment "A metric to measure the legacy support presence dimension of a dataset"@en ;
	rdfs:label "Legacy support presence metric"@en ;
	dqv:inDimension :LegacySupportPresenceDimension .

:LegacySupportDescriptionMetric rdf:type dqv:Metric ;
	rdfs:comment "A metric to measure the legacy support description dimension of a dataset"@en ;
	rdfs:label "Legacy support description metric"@en ;
	dqv:inDimension :LegacySupportDescriptionDimension .


# Augmentation mechanism
:AugmentationPossibilityPresenceDimension rdf:type dqv:Dimension ;
	terms:source "Datasheets for datasets, https://arxiv.org/pdf/1803.09010."@en ;
	rdfs:comment "Indicates whether there is a mechanism through which other may extend/augment/build on / contribute to the dataset"@en ;
	rdfs:label "Augmentation possibility"@en .

:AugmentationPossibilityDescriptionDimension rdf:type dqv:Dimension ;
	terms:source "Datasheets for datasets, https://arxiv.org/pdf/1803.09010."@en ;
	rdfs:comment "Description of how others may extend/augment/build on / contribute to the dataset, if applicable"@en ;
	rdfs:label "Augmentation possibility description"@en .

:AugmentationValidationPresenceDimension rdf:type dqv:Dimension ;
	terms:source "Datasheets for datasets, https://arxiv.org/pdf/1803.09010."@en ;
	rdfs:comment "Indicates whether contributions to the dataset will be validated/verified, if applicable"@en ;
	rdfs:label "Augmentation validation"@en .

# N.B. also needs to be filled out if no validation is carried out
:AugmentationValidationDescriptionDimension rdf:type dqv:Dimension ;
	terms:source "Datasheets for datasets, https://arxiv.org/pdf/1803.09010."@en ;
	rdfs:comment "Description of how contributions to the dataset will be validated/verified, or why it will not be validated/verified, if applicable"@en ;
	rdfs:label "Augmentation validation description"@en .

:AugmentationCommunicationPresenceDimension rdf:type dqv:Dimension ;
	terms:source "Datasheets for datasets, https://arxiv.org/pdf/1803.09010."@en ;
	rdfs:comment "Indicates whether there is a process for communicating / distributing contributions to dataset consumers"@en ;
	rdfs:label "Augmentation communication"@en .

:AugmentationCommunicationDescriptionDimension rdf:type dqv:Dimension ;
	terms:source "Datasheets for datasets, https://arxiv.org/pdf/1803.09010."@en ;
	rdfs:comment "Description of the process for communicating / distributing contributions to dataset consumers"@en ;
	rdfs:label "Augmentation communication description"@en .

:AugmentationPossibilityPresenceMetric rdf:type dqv:Metric ;
	rdfs:comment "A metric to measure the augmentation possibility presence dimension of a dataset"@en ;
	rdfs:label "Augmentation possibility presence metric"@en ;
	dqv:inDimension :AugmentationPossibilityPresenceDimension .

:AugmentationPossibilityDescriptionMetric rdf:type dqv:Metric ;
	rdfs:comment "A metric to measure the augmentation possibility description dimension of a dataset"@en ;
	rdfs:label "Augmentation possibility description metric"@en ;
	dqv:inDimension :AugmentationPossibilityDescriptionDimension .

:AugmentationValidationPresenceMetric rdf:type dqv:Metric ;
	rdfs:comment "A metric to measure the augmentation validation presence dimension of a dataset"@en ;
	rdfs:label "Augmentation validation presence metric"@en ;
	dqv:inDimension :AugmentationValidationPresenceDimension .

:AugmentationValidationDescriptionMetric rdf:type dqv:Metric ;
	rdfs:comment "A metric to measure the augmentation validation description dimension of a dataset"@en ;
	rdfs:label "Augmentation validation description metric"@en ;
	dqv:inDimension :AugmentationValidationDescriptionDimension .

:AugmentationCommunicationPresenceMetric rdf:type dqv:Metric ;
	rdfs:comment "A metric to measure the augmentation communication presence dimension of a dataset"@en ;
	rdfs:label "Augmentation communication presence metric"@en ;
	dqv:inDimension :AugmentationCommunicationPresenceDimension .

:AugmentationCommunicationDescriptionMetric rdf:type dqv:Metric ;
	rdfs:comment "A metric to measure the augmentation communication description dimension of a dataset"@en ;
	rdfs:label "Augmentation communication description metric"@en ;
	dqv:inDimension :AugmentationCommunicationDescriptionDimension .

